All commits merged into one! Includes arm8_strspn, PILbox32, Picinae_numbers, theorem addition, funccall playground

Examples/funccalls/too_complicated/mylib.c
@@ -1,0 +1,47 @@
+unsigned int my_add(unsigned int a, unsigned int b) {
+  while (a > 0) {
+    a = a - 1;
+    b = b + 1;
+  }
+  return b;
+}
+
+unsigned int my_id(unsigned int a) {
+  return my_add(a,0);
+}
+
+unsigned int my_add_rec(unsigned int a, unsigned int b) {
+  if(a==0) return b;
+  return my_add_rec(a-1,b+1);
+}
+
+unsigned int my_add_rec3(unsigned int a, unsigned int b) {
+  if(a==0) return b;
+  if(a>=3) return my_add_rec3(a-3,b+3);
+  return my_add_rec3(a-1,b+1);
+}
+
+void my_add_ptr(unsigned int a, unsigned int *b) {
+  *b = *b + a;
+}
+
+unsigned int factorial(unsigned int a) {
+  unsigned int acc = 1;
+  for(int i = 1; i <= a; i += 1)
+    acc *= i;
+  return acc;
+}
+
+unsigned int recfactorial(unsigned int a) {
+  if (a <= 1) return 1;
+  return a * recfactorial(a-1);
+}
+
+unsigned int factorial_rec_acc_impl(unsigned int a, unsigned int acc){
+  if(a<=1) return acc;
+  return factorial_rec_acc_impl(a-1,acc*a);
+}
+
+unsigned int factorial_rec_acc(unsigned int a){
+  return factorial_rec_acc_impl(a,1);
+}
