Picinae_theory_BACKUP_229760.v
@@ -224,96 +224,6 @@ Proof.
 Qed.
 
 
-Section Functional_choice.
-
-Definition fchoose {A B} (f:A->bool) (g h:A->B) (x:A) :=
-  if f x then h x else g x.
-
-Theorem fchoose_comm:
-  forall {A B} f (g h:A->B), fchoose f g h = fchoose (Basics.compose negb f) h g.
-Proof.
-  intros. extensionality x. unfold fchoose, Basics.compose. destruct (f x); reflexivity.
-Qed.
-
-Theorem fchoose_sup_l:
-  forall {A B} f1 f2 (g h:A->B), (forall x, Bool.le (f1 x) (f2 x)) ->
-  fchoose f1 (fchoose f2 g h) h = fchoose f2 g h.
-Proof.
-  intros. extensionality x. specialize (H x). unfold fchoose. destruct (f1 x).
-    destruct (f2 x). reflexivity. discriminate.
-    reflexivity.
-Qed.
-
-Theorem fchoose_sup_r:
-  forall {A B} f1 f2 (g h:A->B), (forall x, Bool.le (f2 x) (f1 x)) ->
-  fchoose f1 g (fchoose f2 g h) = fchoose f2 g h.
-Proof.
-  intros. extensionality x. specialize (H x). unfold fchoose. destruct (f1 x).
-    reflexivity.
-    destruct (f2 x). discriminate. reflexivity.
-Qed.
-
-Theorem fchoose_revert:
-  forall {A B} f (g h:A->B),
-  fchoose f g (fchoose f h g) = g.
-Proof.
-  intros. extensionality v. unfold fchoose. destruct (f v); reflexivity.
-Qed.
-
-Theorem fchoose_overwrite_l:
-  forall {A B} f (g h h':A->B),
-  fchoose f (fchoose f g h) h' = fchoose f g h'.
-Proof.
-  intros. extensionality x. unfold fchoose. destruct (f x); reflexivity.
-Qed.
-
-Theorem fchoose_overwrite_r:
-  forall {A B} f (g h h':A->B),
-  fchoose f g (fchoose f h h') = fchoose f g h'.
-Proof.
-  intros. extensionality x. unfold fchoose. destruct (f x); reflexivity.
-Qed.
-
-Theorem fchoose_update_distr:
-  forall {A B} {eq:EqDec A} f g h (x:A) (y:B),
-  (fchoose f g h)[x:=y] = fchoose f (g[x:=y]) (h[x:=y]).
-Proof.
-  intros. extensionality x'. unfold fchoose. destruct (x' == x).
-    subst x'. rewrite update_updated. symmetry. destruct (f x); apply update_updated.
-    rewrite update_frame by assumption. symmetry. destruct (f x'); apply update_frame; assumption.
-Qed.
-
-Theorem fchoose_update_l:
-  forall {A B} {eq:EqDec A} f g h (x:A) (y:B), f x = true ->
-  fchoose f (g[x:=y]) h = fchoose f g h.
-Proof.
-  intros. unfold fchoose. extensionality x'. destruct (x' == x).
-    subst x'. rewrite H. reflexivity.
-    destruct (f x'). reflexivity. apply update_frame. assumption.
-Qed.
-
-Theorem fchoose_update_r:
-  forall {A B} {eq:EqDec A} f g h (x:A) (y:B), f x = false ->
-  fchoose f g (h[x:=y]) = fchoose f g h.
-Proof.
-  intros. unfold fchoose. extensionality x'. destruct (x' == x).
-    subst x'. rewrite H. reflexivity.
-    destruct (f x'). apply update_frame. assumption. reflexivity.
-Qed.
-
-Theorem fchoose_update_c:
-  forall {A B} {eq:EqDec A} f g h (x:A) b (y:B),
-  (fchoose (f[x:=b]) g h)[x:=y] = (fchoose f g h)[x:=y].
-Proof.
-  intros. extensionality x'. destruct (x' == x).
-    subst x'. rewrite !update_updated. reflexivity.
-    unfold fchoose. rewrite !update_frame by assumption. reflexivity.
-Qed.
-
-End Functional_choice.
-
-
-
 Section NInduction.
 
 (* Analogues of theorems about Pos.iter, but for N.iter. *)
@@ -4576,7 +4486,49 @@ Tactic Notation "focus_addr" constr(n) :=
                               | _ => idtac end).
 
 
+<<<<<<< HEAD
 Section MemTheory.
+=======
+
+Module Type PICINAE_THEORY (IL: PICINAE_IL).
+
+Import IL.
+Open Scope N.
+
+(* Define an alternative inductive principle for structural inductions on stmts
+   that works better for proving properties of *executed* stmts that might contain
+   repeat-loops.  The cases for all non-repeat forms are the same as Coq's default
+   stmt_ind principle, but properties P of repeat-loops are provable from assuming
+   that the expansion of the loop into a sequence satisfies P.
+ *)
+Theorem stmt_ind2 (P: stmt -> Prop):
+  P Nop ->
+  (forall v e, P (Move v e)) ->
+  (forall e, P (Jmp e)) ->
+  (forall i, P (Exn i)) ->
+  (forall q1 q2 (IHq1: P q1) (IHq2: P q2), P (Seq q1 q2)) ->
+  (forall e q1 q2 (IHq1: P q1) (IHq2: P q2), P (If e q1 q2)) ->
+  (forall e q (IHq1: P q) (IHq2: forall n, P (N.iter n (Seq q) Nop)), P (Rep e q)) ->
+  forall (q:stmt), P q.
+Proof.
+  intros. induction q.
+    assumption.
+    apply H0.
+    apply H1.
+    apply H2.
+    apply H3; assumption.
+    apply H4; assumption.
+    apply H5. assumption. apply Niter_invariant.
+      apply H.
+      intros. apply H3; assumption.
+Qed.
+
+
+Notation "x << y" := (N.shiftl x y) (at level 55, left associativity). (* logical shift-left *)
+Notation "x >> y" := (N.shiftr x y) (at level 55, left associativity). (* logical shift-right *)
+
+Section StoreTheory.
+>>>>>>> 4c730b0 (All commits merged into one! Includes arm8_strspn, PILbox32, Picinae_numbers, theorem addition, funccall playground)
 
 (* The getmem/setmem memory accessors are defined as Peano recursions over N,
    rather than natural number recursions.  This is important for keeping proof
@@ -4596,11 +4548,16 @@ Section MemTheory.
    (3) Unfold inductive cases (where len = N.succ _) using the getmem_succ
        or setmem_succ theorems. *)
 
-(* The upper bound for the numeric representation of virtual memory is
-   2^(2^w*8), which is a huge number that Coq must avoid expanding.
-   We therefore create a special name for it here, allowing proof
-   environments to set it Opaque. *)
-Definition memsize w := 2^(2^w*8).
+(* Memory sizes are huge, so make "pow2 x" an unexpanding alias for 2^x. *)
+Theorem memsize_sig: sig (fun pow2 => N.pow 2 = pow2).
+Proof. econstructor. reflexivity. Qed.
+Definition pow2 := proj1_sig memsize_sig.
+Theorem fold_pow2: N.pow 2 = pow2.
+Proof. apply (proj2_sig memsize_sig). Qed.
+
+Definition memsize w := pow2 (8*2^w).
+Theorem fold_memsize: forall w, 2^(8*2^w) = memsize w.
+Proof. unfold memsize. rewrite fold_pow2. reflexivity. Qed.
 
 (* Base cases for getmem/setmem *)
 Theorem getmem_0: forall w e m a, getmem w e N0 m a = N0.
@@ -4612,7 +4569,7 @@ Proof. reflexivity. Qed.
 (* Unfold getmem/setmem by one byte (for inductive cases of proofs). *)
 Theorem getmem_succ:
   forall w e len m a, getmem w e (N.succ len) m a =
-    match e with BigE => N.lor (getmem w e len m (N.succ a)) (N.shiftl (getbyte m a w) (len*8))
+    match e with BigE => N.lor (getmem w e len m (N.succ a)) (N.shiftl (getbyte m a w) (8*len))
                | LittleE => N.lor (getbyte m a w) (N.shiftl (getmem w e len m (N.succ a)) 8)
     end.
 Proof.
@@ -4624,7 +4581,7 @@ Qed.
 
 Theorem setmem_succ:
   forall w e len m a v, setmem w e (N.succ len) m a v =
-    match e with BigE => setmem w e len (setbyte m a (N.shiftr v (len*8)) w) (N.succ a) (v mod 2^(len*8))
+    match e with BigE => setmem w e len (setbyte m a (N.shiftr v (8*len)) w) (N.succ a) (v mod 2^(8*len))
                | LittleE => setmem w e len (setbyte m a v w) (N.succ a) (N.shiftr v 8)
     end.
 Proof.
@@ -4639,7 +4596,7 @@ Qed.
 Corollary getmem_1: forall w e m a, getmem w e 1 m a = getbyte m a w.
 Proof.
   intros. change 1 with (N.succ 0).
-  rewrite getmem_succ, getmem_0, N.mul_0_l, N.shiftl_0_r, N.lor_0_l, N.lor_0_r.
+  rewrite getmem_succ, getmem_0, N.mul_0_r, N.shiftl_0_r, N.lor_0_l, N.lor_0_r.
   destruct e; reflexivity.
 Qed.
 
@@ -4647,34 +4604,34 @@ Corollary setmem_1: forall w e m a v, setmem w e 1 m a v = setbyte m a v w.
 Proof.
   intros.
   change 1 with (N.succ 0).
-  rewrite setmem_succ, !setmem_0, N.mul_0_l, N.shiftr_0_r.
+  rewrite setmem_succ, !setmem_0, N.mul_0_r, N.shiftr_0_r.
   destruct e; reflexivity.
 Qed.
 
 Theorem getbyte_bound:
   forall m a w, getbyte m a w < 2^8.
 Proof.
-  intros. rewrite <- (N.mul_1_l 8), <- (N.add_sub 1 (a mod 2^w)),
-                  N.add_1_l, N.mul_sub_distr_r.
+  intros. rewrite <- (N.mul_1_r 8), <- (N.add_sub 1 (a mod 2^w)),
+                  N.add_1_l, N.mul_sub_distr_l.
   apply xbits_bound.
 Qed.
 
 Theorem getmem_bound:
-  forall w e len m a, getmem w e len m a < 2^(len*8).
+  forall w e len m a, getmem w e len m a < 2^(8*len).
 Proof.
   induction len using N.peano_ind; intros.
     rewrite getmem_0. apply mp2_gt_0.
     rewrite getmem_succ. destruct e; apply lor_bound.
       eapply N.lt_le_trans. apply IHlen. apply N.pow_le_mono_r.
         discriminate 1.
-        apply N.mul_le_mono_r, N.le_succ_diag_r.
-      rewrite N.mul_succ_l, N.add_comm. apply shiftl_bound, getbyte_bound.
+        apply N.mul_le_mono_l, N.le_succ_diag_r.
+      rewrite N.mul_succ_r, N.add_comm. apply shiftl_bound, getbyte_bound.
       eapply N.lt_le_trans.
         apply mp2_mod_lt.
         apply N.pow_le_mono_r. discriminate 1.
-          rewrite <- N.mul_sub_distr_r, <- N.add_1_l, N.add_sub, <- N.add_1_l.
-          apply N.mul_le_mono. apply N.le_add_r. reflexivity.
-      rewrite N.mul_succ_l. apply shiftl_bound, IHlen.
+          rewrite <- N.mul_sub_distr_l, <- N.add_1_l, N.add_sub, <- N.add_1_l.
+          apply N.mul_le_mono. reflexivity. apply N.le_add_r.
+      rewrite N.mul_succ_r. apply shiftl_bound, IHlen.
 Qed.
 
 Theorem getbyte_mod_l:
@@ -4713,7 +4670,7 @@ Proof.
 Qed.
 
 Theorem getmem_mod_r:
-  forall w e len m a, (getmem w e len m a) mod 2^(len*8) = getmem w e len m a.
+  forall w e len m a, (getmem w e len m a) mod 2^(8*len) = getmem w e len m a.
 Proof.
   intros. apply N.mod_small. apply getmem_bound.
 Qed.
@@ -4746,51 +4703,51 @@ Qed.
 
 Theorem setmem_mod_r:
   forall w e len m a v,
-  setmem w e len m a (v mod 2^(len*8)) = setmem w e len m a v.
+  setmem w e len m a (v mod 2^(8*len)) = setmem w e len m a v.
 Proof.
   induction len using N.peano_ind; intros.
     rewrite !setmem_0. reflexivity.
     rewrite !setmem_succ. destruct e.
 
       rewrite <- xbits_equiv. unfold xbits.
-      rewrite <- N.mul_sub_distr_r, <- N.add_1_l, N.add_sub, N.mul_1_l at 1.
+      rewrite <- N.mul_sub_distr_l, <- N.add_1_l, N.add_sub, N.mul_1_r at 1.
       rewrite setbyte_mod_r, mp2_mod_mod_min, N.min_r. reflexivity.
-      apply N.mul_le_mono_r, N.le_succ_diag_r.
+      apply N.mul_le_mono_l, N.le_succ_diag_r.
 
       rewrite <- setbyte_mod_r, mp2_mod_mod_min, N.min_r, setbyte_mod_r.
-        rewrite <- xbits_equiv. unfold xbits. rewrite N.mul_comm, <- N.mul_pred_r, N.pred_succ, N.mul_comm. apply IHlen.
-        rewrite N.mul_succ_l. apply N.le_add_l.
+        rewrite <- xbits_equiv. unfold xbits. rewrite <- N.mul_pred_r, N.pred_succ. apply IHlen.
+        rewrite N.mul_succ_r, N.add_comm. apply N.le_add_r.
 Qed.
 
 (* Break an (i+j)-byte number read/stored to/from memory into two numbers of size i and j. *)
 Theorem getmem_split:
   forall w e i j m a, getmem w e (i+j) m a =
-    match e with BigE => N.lor (getmem w e j m (a+i)) (N.shiftl (getmem w e i m a) (j*8))
-               | LittleE => N.lor (getmem w e i m a) (N.shiftl (getmem w e j m (a+i)) (i*8))
+    match e with BigE => N.lor (getmem w e j m (a+i)) (N.shiftl (getmem w e i m a) (8*j))
+               | LittleE => N.lor (getmem w e i m a) (N.shiftl (getmem w e j m (a+i)) (8*i))
     end.
 Proof.
   induction i using N.peano_ind; intros.
-    rewrite N.add_0_l, N.add_0_r, N.mul_0_l, getmem_0, N.shiftl_0_l, N.shiftl_0_r, N.lor_0_r, N.lor_0_l. destruct e; reflexivity.
+    rewrite N.add_0_l, N.add_0_r, N.mul_0_r, getmem_0, N.shiftl_0_l, N.shiftl_0_r, N.lor_0_r, N.lor_0_l. destruct e; reflexivity.
     rewrite <- N.add_succ_comm, getmem_succ, N.add_succ_l. destruct e.
-      rewrite N.shiftl_lor, N.shiftl_shiftl, N.lor_assoc, <- IHi, <- N.mul_add_distr_r. apply getmem_succ.
-      rewrite (N.mul_succ_l i), <- N.shiftl_shiftl, <- N.lor_assoc, <- N.shiftl_lor, <- IHi. apply getmem_succ.
+      rewrite N.shiftl_lor, N.shiftl_shiftl, N.lor_assoc, <- IHi, <- N.mul_add_distr_l. apply getmem_succ.
+      rewrite (N.mul_succ_r _ i), <- N.shiftl_shiftl, <- N.lor_assoc, <- N.shiftl_lor, <- IHi. apply getmem_succ.
 Qed.
 
 Theorem setmem_split:
   forall w e i j m a v, setmem w e (i+j) m a v =
-    match e with BigE => setmem w e j (setmem w e i m a (N.shiftr v (j*8))) (a+i) v
-               | LittleE => setmem w e j (setmem w e i m a (v mod 2^(i*8))) (a+i) (N.shiftr v (i*8))
+    match e with BigE => setmem w e j (setmem w e i m a (N.shiftr v (8*j))) (a+i) v
+               | LittleE => setmem w e j (setmem w e i m a (v mod 2^(8*i))) (a+i) (N.shiftr v (8*i))
     end.
 Proof.
   induction i using N.peano_ind; intros.
     rewrite N.add_0_r, N.shiftr_0_r, !setmem_0. destruct e; reflexivity.
     rewrite N.add_succ_comm. rewrite IHi. rewrite !(setmem_succ _ _ j). destruct e.
 
-      erewrite <- setmem_1, <- N.add_1_r, N.mul_add_distr_r, <- N.shiftr_shiftr, <- IHi.
+      erewrite <- setmem_1, <- N.add_1_r, N.mul_add_distr_l, <- N.shiftr_shiftr, <- IHi.
       rewrite N.add_1_r, N.add_succ_r. apply setmem_mod_r.
 
       erewrite <- setmem_1, <- IHi, N.add_succ_r, N.add_1_r, setmem_mod_r.
-      rewrite N.shiftr_shiftr, N.mul_succ_l. reflexivity.
+      rewrite N.shiftr_shiftr, N.mul_succ_r. reflexivity.
 Qed.
 
 Lemma getmem_shiftr8__getmem':
@@ -4825,7 +4782,7 @@ Qed.
 
 Theorem getmem_mod:
   forall w e n2 n1 m a,
-    (getmem w e n1 m a) mod 2^(n2*8) = getmem w e (N.min n1 n2) m
+    (getmem w e n1 m a) mod 2^(8*n2) = getmem w e (N.min n1 n2) m
       match e with BigE => a + (n1 - n2) | LittleE => a end.
 Proof.
   intros. destruct (N.le_ge_cases n1 n2).
@@ -4834,7 +4791,7 @@ Proof.
     replace (match e with BigE => _ | _ => _ end) with a by (destruct e; reflexivity).
     apply N.mod_small. eapply N.lt_le_trans.
       apply getmem_bound.
-      apply N.pow_le_mono_r. discriminate 1. apply N.mul_le_mono_r. assumption.
+      apply N.pow_le_mono_r. discriminate 1. apply N.mul_le_mono_l. assumption.
 
     rewrite N.min_r, <- N.land_ones by assumption. destruct e;
       [ rewrite <- (N.sub_add _ _ H) at 1
@@ -4846,14 +4803,14 @@ Qed.
 
 Theorem shiftr_getmem:
   forall w e n2 n1 m a,
-  N.shiftr (getmem w e n1 m a) (n2*8) = getmem w e (n1-n2) m
+  N.shiftr (getmem w e n1 m a) (8*n2) = getmem w e (n1-n2) m
     match e with BigE => a | LittleE => a + n2 end.
 Proof.
   intros. destruct (N.le_ge_cases n1 n2).
 
     rewrite (proj2 (N.sub_0_le _ _)), getmem_0 by assumption. eapply shiftr_low_pow2, N.lt_le_trans.
       apply getmem_bound.
-      apply N.pow_le_mono_r. discriminate 1. apply N.mul_le_mono_r. assumption.
+      apply N.pow_le_mono_r. discriminate 1. apply N.mul_le_mono_l. assumption.
 
     destruct e;
     [ rewrite <- (N.sub_add _ _ H) at 1
@@ -4864,9 +4821,9 @@ Qed.
 
 Theorem getbyte_spec:
   forall m a w i, N.testbit (getbyte m a w) i =
-    andb (N.testbit m ((a mod 2^w)*8 + i)) (i <? 8).
+    andb (N.testbit m (8*(a mod 2^w) + i)) (i <? 8).
 Proof.
-  intros. unfold getbyte. rewrite xbits_spec, N.add_comm, N.mul_succ_l.
+  intros. unfold getbyte. rewrite xbits_spec, N.add_comm, N.mul_succ_r.
   apply f_equal. destruct (_ <? _) eqn:H; symmetry.
     eapply N.ltb_lt, N.add_lt_mono_l, N.ltb_lt, H.
     eapply N.ltb_ge, N.add_le_mono_l, N.ltb_ge, H.
@@ -4874,8 +4831,8 @@ Qed.
 
 Theorem setbyte_spec:
   forall m a v w i, N.testbit (setbyte m a v w) i =
-    if andb ((a mod 2^w)*8 <=? i) (i <? N.succ(a mod 2^w)*8)
-    then N.testbit v (i - (a mod 2^w)*8) else N.testbit m i.
+    if andb (8*(a mod 2^w) <=? i) (i <? 8*N.succ(a mod 2^w))
+    then N.testbit v (i - 8*(a mod 2^w)) else N.testbit m i.
 Proof.
   intros. unfold setbyte. rewrite N.lor_spec, N.ldiff_spec, <- (N.land_ones v).
   destruct (_ <=? _) eqn:H1.
@@ -4885,12 +4842,12 @@ Proof.
       rewrite N.ones_spec_low.
         rewrite Bool.andb_false_r, Bool.andb_true_r. reflexivity.
         eapply N.add_lt_mono_r. rewrite N.sub_add.
-          rewrite N.add_comm, <- N.mul_succ_l. apply N.ltb_lt, H2.
+          rewrite N.add_comm, <- N.mul_succ_r. apply N.ltb_lt, H2.
           apply N.leb_le, H1.
       rewrite N.ones_spec_high.
         rewrite Bool.andb_false_r, Bool.andb_true_r. apply Bool.orb_false_r.
         eapply N.add_le_mono_r. rewrite N.sub_add.
-          rewrite N.add_comm, <- N.mul_succ_l. apply N.ltb_ge, H2.
+          rewrite N.add_comm, <- N.mul_succ_r. apply N.ltb_ge, H2.
           apply N.leb_le, H1.
 
     rewrite !N.shiftl_spec_low by apply N.leb_gt, H1.
@@ -4910,12 +4867,12 @@ Proof.
         reflexivity.
         eapply N.lt_le_trans.
           apply N.add_lt_mono_l, H1.
-          rewrite <- N.mul_succ_l. apply N.mul_le_mono_r, N.le_succ_l, NE.
+          rewrite <- N.mul_succ_r. apply N.mul_le_mono_l, N.le_succ_l, NE.
       rewrite (proj2 (N.ltb_ge _ _)).
         rewrite Bool.andb_false_r. reflexivity.
         etransitivity.
-          apply N.mul_le_mono_r, N.le_succ_l, NE.
-          rewrite N.mul_comm. apply N.le_add_r.
+          apply N.mul_le_mono_l, N.le_succ_l, NE.
+          apply N.le_add_r.
 
     rewrite !Bool.andb_false_r. reflexivity.
 Qed.
@@ -4927,14 +4884,14 @@ Proof.
   intros. unfold getbyte, setbyte. rewrite EQ.
   rewrite xbits_lor, xbits_ldiff, !xbits_shiftl, xbits_ones.
   rewrite N.sub_diag, !N.shiftl_0_r, N.sub_0_r.
-  rewrite <- N.mul_sub_distr_r, <- N.add_1_l, N.add_sub, N.mul_1_l.
+  rewrite <- N.mul_sub_distr_l, <- N.add_1_l, N.add_sub, N.mul_1_r.
   rewrite N.min_id, xbits_0_i, mp2_mod_mod.
   set (x := xbits _ _ _). destruct (N.eq_0_gt_0_cases x) as [H|H].
     rewrite H, N.ldiff_0_l. apply N.lor_0_l.
     rewrite N.ldiff_ones_r_low.
       apply N.lor_0_l.
       apply N.log2_lt_pow2. apply H.
-        erewrite <- (N.mul_1_l 8), <- (N.add_sub 1), N.mul_sub_distr_r.
+        erewrite <- (N.mul_1_r 8), <- (N.add_sub 1), N.mul_sub_distr_l.
         apply xbits_bound.
 Qed.
 
@@ -4958,7 +4915,7 @@ Qed.
 
 Theorem setmem_highbits:
   forall w e len m a v,
-  N.shiftr (setmem w e len m a v) (2^w*8) = N.shiftr m (2^w*8).
+  N.shiftr (setmem w e len m a v) (8*2^w) = N.shiftr m (8*2^w).
 Proof.
   induction len using N.peano_ind; intros.
     rewrite setmem_0. reflexivity.
@@ -4966,7 +4923,7 @@ Proof.
      (rewrite !N.shiftr_spec', setbyte_spec, (proj2 (N.ltb_ge _ _));
       [ rewrite Bool.andb_false_r; reflexivity
       | etransitivity; [|apply N.le_add_l];
-          apply N.mul_le_mono_r, N.le_succ_l, mp2_mod_lt ]).
+          apply N.mul_le_mono_l, N.le_succ_l, mp2_mod_lt ]).
 Qed.
 
 (* getmem doesn't read addresses outside the interval [a, a+len). *)
@@ -5015,36 +4972,36 @@ Qed.
 Lemma setmem_frame_byte:
   forall a' w en len m a n
     (LE: a' < 2^w -> len <= msub w a' a),
-  xbits (setmem w en len m a n) (a' * 8) (N.succ a' * 8) =
-  xbits m (a' * 8) (N.succ a' * 8).
+  xbits (setmem w en len m a n) (8*a') (8*N.succ a') =
+  xbits m (8*a') (8*N.succ a').
 Proof.
   intros. destruct (N.lt_ge_cases a' (2^w)).
 
     rewrite <- (N.mod_small _ _ H). apply setmem_frame. apply LE, H.
 
-    rewrite <- (recompose_bytes (2^w*8) (setmem _ _ _ _ _ _)).
+    rewrite <- (recompose_bytes (8*2^w) (setmem _ _ _ _ _ _)).
     rewrite setmem_highbits, !xbits_lor.
     rewrite xbits_above, N.lor_0_l.
 
-      rewrite xbits_shiftl, <- !N.mul_sub_distr_r.
-      rewrite (proj2 (N.sub_0_le _ _) H), N.mul_0_l, N.shiftl_0_r.
-      rewrite xbits_shiftr, <- !N.mul_add_distr_r, !N.sub_add. reflexivity.
+      rewrite xbits_shiftl, <- !N.mul_sub_distr_l.
+      rewrite (proj2 (N.sub_0_le _ _) H), N.mul_0_r, N.shiftl_0_r.
+      rewrite xbits_shiftr, <- !N.mul_add_distr_l, !N.sub_add. reflexivity.
         etransitivity. apply H. apply N.le_succ_r. left. reflexivity.
         apply H.
 
       eapply N.lt_le_trans. apply mp2_mod_lt.
       apply N.pow_le_mono_r. discriminate.
-      apply N.mul_le_mono_r, H.
+      apply N.mul_le_mono_l, H.
 Qed.
 
 (* getmem inverts setmem *)
 Theorem getmem_setmem:
   forall w e len m a v (LE: len <= 2^w),
-  getmem w e len (setmem w e len m a v) a = v mod 2^(len*8).
+  getmem w e len (setmem w e len m a v) a = v mod 2^(8*len).
 Proof.
   intros until len. revert len w.
   induction len using N.peano_ind; intros.
-    rewrite N.mul_0_l, N.mod_1_r. apply getmem_0.
+    rewrite N.mul_0_r, N.mod_1_r. apply getmem_0.
 
     assert (LE': len <= msub w a (N.succ a)).
       rewrite <- N.add_1_r, msub_add_distr, msub_diag, msub_0_l by reflexivity.
@@ -5059,15 +5016,15 @@ Proof.
       rewrite IHlen by (etransitivity; [ apply N.le_succ_diag_r | exact LE ]);
       rewrite setmem_frame by apply LE';
       rewrite getbyte_setbyte by reflexivity.
-        rewrite mp2_mod_mod, <- xbits_split_0, N.mul_succ_l. apply xbits_0_i.
-        rewrite <- xbits_split_0, N.mul_succ_l, N.add_comm. apply xbits_0_i.
+        rewrite mp2_mod_mod, <- xbits_split_0, N.mul_succ_r. apply xbits_0_i.
+        rewrite <- xbits_split_0, N.mul_succ_r, N.add_comm. apply xbits_0_i.
 Qed.
 
 Theorem setmem_byte_anylen:
   forall w en len i m a v (ILE: i < len),
-  getbyte (setmem w en len m a v) (a+i) w = N.shiftr v (
+  getbyte (setmem w en len m a v) (a+i) w = N.shiftr v (8 *
     match en with BigE => msub w (N.pred len) i
-                | LittleE => i + N.pred(len-i)/2^w*2^w end * 8) mod (2^8).
+                | LittleE => i + N.pred(len-i)/2^w*2^w end) mod (2^8).
 Proof.
   intros.
   set (r := N.succ (msub w (N.pred len) i)).
@@ -5113,8 +5070,8 @@ Qed.
 
 Corollary setmem_byte:
   forall w en len i m a v (ILE: i < len) (LEN: len <= 2^w),
-  getbyte (setmem w en len m a v) (a+i) w = N.shiftr v (
-    match en with BigE => N.pred len - i | LittleE => i end * 8) mod (2^8).
+  getbyte (setmem w en len m a v) (a+i) w = N.shiftr v (8 *
+    match en with BigE => N.pred len - i | LittleE => i end) mod (2^8).
 Proof.
   intros. rewrite setmem_byte_anylen by assumption.
   assert (H: N.pred len < 2^w).
@@ -5135,14 +5092,14 @@ Qed.
 
 Theorem setmem_anybyte_anylen:
   forall a' w en len m a v,
-    xbits (setmem w en len m a v) (a' * 8) (N.succ a' * 8) =
+    xbits (setmem w en len m a v) (8*a') (8*N.succ a') =
     if ((msub w a' a <? len) && (a' <? 2^w))%bool then
-      N.shiftr v (
+      N.shiftr v (8 *
         match en with
         | BigE => msub w (a + N.pred len) a'
         | LittleE => msub w a' a + N.pred (len - msub w a' a) / 2^w * 2^w
-        end * 8) mod 2^8
-    else xbits m (a' * 8) (N.succ a' * 8).
+        end) mod 2^8
+    else xbits m (8*a') (8*N.succ a').
 Proof.
   intros. destruct andb eqn:H.
 
@@ -5160,7 +5117,7 @@ Qed.
 Theorem getmem_setmem_xbits:
   forall w en len i j m a v (LE: j + len <= 2^w),
   getmem w en len (setmem w en (i+len+j) m a v) (a+i) =
-  match en with BigE => xbits v (j*8) ((j+len)*8) | LittleE => xbits v (i*8) ((i+len)*8) end.
+  match en with BigE => xbits v (8*j) (8*(j+len)) | LittleE => xbits v (8*i) (8*(i+len)) end.
 Proof.
   intros.
   assert (H1: len <= len mod 2^w \/ j = 0). destruct j as [|j].
@@ -5182,9 +5139,9 @@ Proof.
   | rewrite madd_add_simpl_l_l, add_msub_l; assumption
   | rewrite madd_add_simpl_l_l, msub_add_distr, msub_diag; assumption ] ).
 
-    unfold xbits. rewrite <- N.mul_sub_distr_r, N.add_comm, N.add_sub. reflexivity.
+    unfold xbits. rewrite <- N.mul_sub_distr_l, N.add_comm, N.add_sub. reflexivity.
 
-    rewrite N.add_comm, N.mul_add_distr_r, <- xbits_equiv. unfold xbits.
+    rewrite N.add_comm, N.mul_add_distr_l, <- xbits_equiv. unfold xbits.
     rewrite N.add_sub, mp2_mod_mod. reflexivity.
 Qed.
 
@@ -5192,14 +5149,14 @@ Theorem setmem_merge:
   forall w e i j m a v1 v2,
   setmem w e j (setmem w e i m a v1) (a+i) v2 =
   setmem w e (i+j) m a match e with
-                       | BigE => cbits v1 (j*8) (v2 mod 2^(j*8))
-                       | LittleE => cbits v2 (i*8) (v1 mod 2^(i*8))
+                       | BigE => cbits v1 (8*j) (v2 mod 2^(8*j))
+                       | LittleE => cbits v2 (8*i) (v1 mod 2^(8*i))
                        end.
 Proof.
   symmetry.
   assert (H:=setmem_split w e i j m a). destruct e;
-  [ specialize (H (cbits v1 (j*8) (v2 mod 2^(j*8))))
-  | specialize (H (cbits v2 (i*8) (v1 mod 2^(i*8)))) ];
+  [ specialize (H (cbits v1 (8*j) (v2 mod 2^(8*j))))
+  | specialize (H (cbits v2 (8*i) (v1 mod 2^(8*i)))) ];
   rewrite shiftr_cbits, <- (setmem_mod_r _ _ j), cbits_mod, !setmem_mod_r in H by apply mp2_mod_lt;
   apply H.
 Qed.
@@ -5615,9 +5572,9 @@ Qed.
 Theorem getbyte_mod_mem:
   forall m a w, getbyte (m mod (memsize w)) a w = getbyte m a w.
 Proof.
-  intros. unfold getbyte, memsize.
+  intros. rewrite <- fold_memsize. unfold getbyte.
   rewrite xbits_equiv, mp2_mod_mod_min, N.min_r, <- xbits_equiv. reflexivity.
-  apply N.mul_le_mono_r, N.le_succ_l, mp2_mod_lt.
+  apply N.mul_le_mono_l, N.le_succ_l, mp2_mod_lt.
 Qed.
 
 Theorem byte_equivalent:
@@ -5625,35 +5582,35 @@ Theorem byte_equivalent:
   m1 mod (memsize w) = m2 mod (memsize w).
 Proof.
   intros.
-  apply N.bits_inj. intro i. destruct (N.lt_ge_cases i (2^w*8)) as [H|H].
+  apply N.bits_inj. intro i. destruct (N.lt_ge_cases i (8*2^w)) as [H|H].
 
     rewrite <- (Bool.andb_true_r (N.testbit (m1 mod _) _)), <- (Bool.andb_true_r (N.testbit (m2 mod _) _)).
-    replace true with (i <? N.succ ((i/8) mod 2^w) * 8).
+    replace true with (i <? 8 * N.succ ((i/8) mod 2^w)).
     rewrite (N.div_mod' i 8), N.add_comm.
     rewrite <- !xbits_spec.
-    rewrite N.add_comm, <- N.div_mod', (N.mul_comm 8).
-    rewrite <- (N.mod_small (i/8) (2^w)) by (apply N.Div0.div_lt_upper_bound; rewrite N.mul_comm; apply H).
+    rewrite N.add_comm, <- N.div_mod'.
+    rewrite <- (N.mod_small (i/8) (2^w)) by apply N.Div0.div_lt_upper_bound, H.
     rewrite mp2_mod_mod.
     change (xbits (m1 mod _) _ _) with (getbyte (m1 mod memsize w) (i/8) w).
     rewrite getbyte_mod_mem, EQ, <- getbyte_mod_mem. reflexivity.
 
-      apply N.ltb_lt. rewrite N.mod_small by (apply N.Div0.div_lt_upper_bound; rewrite N.mul_comm; apply H).
-      rewrite (N.div_mod' i 8) at 1. rewrite N.mul_succ_l, (N.mul_comm 8).
+      apply N.ltb_lt. rewrite N.mod_small by apply N.Div0.div_lt_upper_bound, H.
+      rewrite (N.div_mod' i 8) at 1. rewrite N.mul_succ_r.
       apply N.add_lt_mono_l, N.mod_lt. discriminate.
 
-    unfold memsize. rewrite !N.mod_pow2_bits_high by apply H. reflexivity.
+    rewrite <- fold_memsize. rewrite !N.mod_pow2_bits_high by apply H. reflexivity.
 Qed.
 
 Theorem bytes_inj:
   forall m1 m2
-    (EQ: forall a, xbits m1 (a*8) (N.succ a * 8) = xbits m2 (a*8) (N.succ a * 8)),
+    (EQ: forall a, xbits m1 (8*a) (8*N.succ a) = xbits m2 (8*a) (8*N.succ a)),
   m1 = m2.
 Proof.
   intros. apply N.bits_inj. intro i.
-  rewrite (N.div_mod' i 8), N.mul_comm, N.add_comm, <- !N.shiftr_spec'.
+  rewrite (N.div_mod' i 8), N.add_comm, <- !N.shiftr_spec'.
   rewrite <- 2!(N.mod_pow2_bits_low (N.shiftr _ _) 8) by apply (mp2_mod_lt _ 3).
   specialize (EQ (i/8)). unfold xbits in EQ.
-  rewrite N.mul_succ_l, (N.add_comm _ 8), N.add_sub in EQ.
+  rewrite N.mul_succ_r, (N.add_comm _ 8), N.add_sub in EQ.
   rewrite EQ. reflexivity.
 Qed.
 
@@ -5664,10 +5621,10 @@ Theorem setmem_swap:
   setmem w e len1 (setmem w e len2 m a2 v2) a1 v1.
 Proof.
   intros.
-  rewrite <- (recompose_bytes (2^w*8) (setmem w e _ _ _ _)). symmetry.
-  rewrite <- (recompose_bytes (2^w*8) (setmem w e _ _ _ _)).
+  rewrite <- (recompose_bytes (8*2^w) (setmem w e _ _ _ _)). symmetry.
+  rewrite <- (recompose_bytes (8*2^w) (setmem w e _ _ _ _)).
   rewrite !setmem_highbits. apply f_equal2; [|reflexivity].
-  apply byte_equivalent. intro a.
+  rewrite fold_memsize. apply byte_equivalent. intro a.
   destruct (overlap_dec w a 1 a1 len1) as [H1|H1].
 
     erewrite overlap_getbyte_updated by assumption.
@@ -5696,8 +5653,8 @@ Theorem setmem_merge_rev:
   forall w e i j m a v1 v2, i + j < 2^w ->
   setmem w e j (setmem w e i m a v2) (msub w a j) v1 =
   setmem w e (i+j) m (msub w a j) match e with
-                                  | BigE => cbits v1 (i*8) (v2 mod 2^(i*8))
-                                  | LittleE => cbits v2 (j*8) (v1 mod 2^(j*8))
+                                  | BigE => cbits v1 (8*i) (v2 mod 2^(8*i))
+                                  | LittleE => cbits v2 (8*j) (v1 mod 2^(8*j))
                                   end.
 Proof.
   intros.
@@ -6151,6 +6108,7 @@ Qed.
 End Determinism.
 
 
+<<<<<<< HEAD
 Section Monotonicity.
 
 (* exec_prog is monotonic with respect to programs.  Enlarging the space of known
@@ -6197,198 +6155,11 @@ Proof.
     apply IHXS, H.
 Qed.
 
-(* eval_exp, exec_stmt, and exec_prog ignore the values of variables not in the
-   typing context. *)
-
-Definition memacc_respects_typctx (c:typctx) :=
-  forall s1 s2, reset_vars c s1 s2 = s1 ->
-  (mem_readable s1 = mem_readable s2) /\
-  (mem_writable s1 = mem_writable s2).
-
-Definition in_ctx (c:typctx) v := if c v then true else false.
-
-Lemma reset_vars_fchoose:
-  forall c, reset_vars c = fchoose (in_ctx c).
-Proof.
-  intros. extensionality s1. extensionality s2. extensionality v.
-  unfold reset_vars, fchoose, in_ctx. destruct (c v); reflexivity.
-Qed.
-
-Lemma reset_vars_sup_l:
-  forall c1 c2 s1 s2
-    (H: forall v, Bool.le (in_ctx c1 v) (in_ctx c2 v)),
-  reset_vars c1 (reset_vars c2 s1 s2) s2 = reset_vars c2 s1 s2.
-Proof.
-  intros. rewrite !reset_vars_fchoose. apply fchoose_sup_l. assumption.
-Qed.
-
-Lemma reset_vars_revert:
-  forall c s s', reset_vars c s' (reset_vars c s s') = s'.
-Proof.
-  intros. rewrite !reset_vars_fchoose. apply fchoose_revert.
-Qed.
-
-Lemma reset_vars_overwrite_l:
-  forall c s1 s2 s3,
-  reset_vars c (reset_vars c s1 s2) s3 = reset_vars c s1 s3.
-Proof.
-  intros. rewrite !reset_vars_fchoose. apply fchoose_overwrite_l.
-Qed.
-
-Lemma reset_vars_overwrite_r:
-  forall c s1 s2 s3,
-  reset_vars c s1 (reset_vars c s2 s3) = reset_vars c s1 s3.
-Proof.
-  intros. rewrite !reset_vars_fchoose. apply fchoose_overwrite_r.
-Qed.
-
-Lemma reset_vars_update_distr:
-  forall c s1 s2 v n,
-  reset_vars c s1 s2[v:=n] = reset_vars c (s1[v:=n]) (s2[v:=n]).
-Proof.
-  intros. rewrite !reset_vars_fchoose. apply fchoose_update_distr.
-Qed.
-
-Lemma reset_vars_update_c:
-  forall c s1 s2 v y n,
-  (reset_vars (c[v:=y]) s1 s2)[v:=n] = (reset_vars c s1 s2)[v:=n].
-Proof.
-  intros. rewrite !reset_vars_fchoose.
-  replace (in_ctx _) with ((in_ctx c)[v:=if y then true else false]).
-  apply fchoose_update_c.
-  extensionality v'. unfold in_ctx. destruct (v' == v).
-    subst v'. rewrite !update_updated. reflexivity.
-    rewrite !update_frame by assumption. reflexivity.
-Qed.
-
-Theorem eval_exp_cframe:
-  forall c (MRC: memacc_respects_typctx c) s1 s2 e n w
-    (RV: reset_vars c s1 s2 = s1)
-    (EE: eval_exp c s1 e n w),
-  eval_exp c s2 e n w.
-Proof.
-  intros. revert s2 RV. dependent induction EE; intros;
-  try (econstructor; try solve [ assumption
-  | (apply IHEE1 + apply IHEE2 + apply IHEE3 + apply IHEE); assumption ]).
-
-    rewrite <- RV. unfold reset_vars. rewrite TYP. apply EVar. assumption.
-    intros n LEN. rewrite <- (proj1 (MRC _ _ RV)). apply R. assumption.
-    intros n LEN. rewrite <- (proj2 (MRC _ _ RV)). apply W. assumption.
-    apply IHEE2.
-      intros s1' s2' RV'. apply MRC. rewrite <- RV'. apply reset_vars_sup_l.
-        intro v'. unfold in_ctx. destruct (v' == v).
-          subst v'. rewrite update_updated. destruct (c v); reflexivity.
-          rewrite update_frame by assumption. destruct (c v'); reflexivity.
-      rewrite <- reset_vars_update_distr, reset_vars_update_c, RV. reflexivity.
-Qed.
-
-Theorem exec_stmt_cframe:
- forall c (MRC: memacc_respects_typctx c) s1 s2 q c' s' x
-   (RV: reset_vars c s1 s2 = s1)
-   (XS: exec_stmt c s1 q c' s' x),
- exec_stmt c s2 q c' (reset_vars c' s2 s') x.
-Proof.
-  intros.
-  revert s2 RV. dependent induction XS; intros;
-    try (rewrite <- RV, reset_vars_revert).
-
-    apply XNop.
-    replace (reset_vars _ _ _) with (s2[v:=n]). apply XMove.
-      eapply eval_exp_cframe; eassumption.
-      extensionality v'. unfold reset_vars. destruct (v' == v).
-        subst v'. rewrite !update_updated. reflexivity.
-        rewrite !update_frame by assumption.
-          destruct (c v') eqn:CV'; [|reflexivity].
-          rewrite update_frame, <- RV by assumption. unfold reset_vars. rewrite CV'. reflexivity.
-    eapply XJmp. eapply eval_exp_cframe; eassumption.
-    apply XExn.
-    apply XSeq1. apply IHXS; assumption.
-
-    eapply XSeq2.
-      apply IHXS1; assumption.
-      eenough (H': reset_vars c' s0 s' = _). rewrite H'. eapply IHXS2.
-
-        intros s1' s2' RV'. apply MRC. extensionality v'.
-        assert (M1:=exec_stmt_cmono v' _ _ _ _ _ _ XS1).
-        unfold reset_vars. destruct (c v') eqn:CV'; [|reflexivity].
-        rewrite <- RV'. unfold reset_vars. destruct (c2 v').
-          reflexivity.
-          discriminate M1. reflexivity.
-
-        extensionality v'.
-        assert (M2:=exec_stmt_cmono v' _ _ _ _ _ _ XS2).
-        unfold reset_vars.
-        destruct (c2 v') eqn:C2V'; [|reflexivity].
-        rewrite C2V'. reflexivity.
-
-        extensionality v'.
-        assert (M2:=exec_stmt_cmono v' _ _ _ _ _ _ XS2).
-        unfold reset_vars.
-        destruct (c' v') eqn:C'V'. reflexivity.
-        rewrite M2; reflexivity.
-
-    eapply XIf.
-      eapply eval_exp_cframe; eassumption.
-      apply IHXS; assumption.
-    eapply XRep.
-      eapply eval_exp_cframe; eassumption.
-      apply IHXS; assumption.
-Qed.
-
-Theorem exec_prog_map:
-  forall f p t
-    (CS: forall xs' xs, can_step p (xs',xs) -> can_step p (f xs', f xs))
-    (XP: exec_prog p t),
-  exec_prog p (map f t).
-Proof.
-  intros. apply Forall_forall. intros (xs',xs) IN'.
-  apply In_ith in IN'. destruct IN' as [i IN'].
-  apply Forall_ith with (i:=i) in XP.
-  destruct (ith (stepsof t) i) as [(xs0',xs0)|] eqn:H.
-
-    rewrite ith_stepsof in IN'.
-    destruct (skipn i _) as [|xs1 l1] eqn:H1. discriminate.
-    destruct l1 as [|xs2 l2] eqn:H2. discriminate.
-    inversion IN'; clear IN'; subst.
-    rewrite skipn_map in H1.
-    rewrite ith_stepsof in H.
-    destruct (skipn i t) as [|xs1' l1'] eqn:H1'. discriminate.
-    destruct l1' as [|xs2' l2'] eqn:H2'. discriminate.
-    inversion H; clear H; subst.
-    inversion H1; clear H1; subst.
-    apply CS. assumption.
-
-    contradict H. apply ith_Some.
-    erewrite length_stepsof, <- map_length, <- length_stepsof.
-    apply ith_Some. rewrite IN'. discriminate.
-Qed.
-
-Theorem exec_prog_cframe:
-  forall p t s0
-    (MRC: memacc_respects_typctx archtyps)
-    (CODEACC: forall s, p s = p (reset_temps s0 s))
-    (XP: exec_prog p t),
-  exec_prog p (map (fun (xs:exit*store) => let (x,s) := xs in
-    (x, reset_temps s0 s)) t).
-Proof.
-  intros. apply exec_prog_map; [|assumption].
-  intros (x',s') (x,s) CS. inversion CS; clear CS; subst.
-
-  eenough (H: reset_temps _ _ = _).
-    rewrite H. eapply CanStep.
-      rewrite <- CODEACC. eassumption.
-      eapply exec_stmt_cframe in XS. exact XS. assumption.
-      apply reset_vars_revert.
-
-    unfold reset_temps.
-    rewrite reset_vars_overwrite_l, reset_vars_overwrite_r.
-    extensionality v. unfold reset_vars.
-    assert (M':=exec_stmt_cmono v _ _ _ _ _ _ XS).
-    destruct (archtyps v) eqn:CV; [|reflexivity].
-    destruct (c' v). reflexivity. discriminate M'. reflexivity.
-Qed.
-
 End Monotonicity.
+
+
+=======
+>>>>>>> 4c730b0 (All commits merged into one! Includes arm8_strspn, PILbox32, Picinae_numbers, theorem addition, funccall playground)
 
 Section InvariantProofs.
 
@@ -7257,7 +7028,7 @@ Proof.
     exact XP.
     simpl. rewrite ENTRY. reflexivity.
     intros. apply (noassign_stmt_same v) in XS.
-      rewrite PRE. simpl. inversion XS. unfold reset_temps, reset_vars. destruct (archtyps v).
+      rewrite PRE. simpl. inversion XS. unfold reset_temps. destruct (archtyps v).
         assumption.
         reflexivity.
       specialize (NA s1 a1). rewrite IL in NA. exact NA.
