Examples/funccalls/loop_nop_proofs.v
@@ -1,0 +1,56 @@
+Require Import Utf8.
+Require Import FunctionalExtensionality.
+Require Import Arith.
+Require Import NArith.
+Require Import ZArith.
+Require Import Picinae_armv8_pcode.
+Require Import nops_o_loop_nop_armv8.
+
+Import ARM8Notations.
+Open Scope N.
+
+Definition loop_nop_exit (t:trace) :=
+  match t with (Addr a, _)::_ => match a with
+  | 0x00100040 => true
+  | _ => false end | _ => false end.
+  
+Definition loop_nop_invs (s0:store) (t:trace) :=
+  match t with (Addr a, s)::_ => match a with
+  | 0x00100030 => Some (arm8equiv_or s s0 (fun v => match v with R_X0 => true | _ => false end))
+  | 0x00100040 => Some (arm8equiv_or s s0 (fun v => match v with R_X0 => true | _ => false end))
+  | _ => None end | _ => None end.
+  
+Theorem loop_nop_pc :
+  forall s t x' s'
+     (ENTRY: startof t (x',s') = (Addr 0x00100030,s))
+     (MDL: models arm8typctx s),
+     satisfies_all loop_nop (loop_nop_invs s) loop_nop_exit ((x',s')::t).
+Proof.
+  Local Ltac step := time arm8_step.
+  intros. 
+  (* Base case *)
+  apply prove_invs. simpl. rewrite ENTRY. step. 
+  unfold arm8equiv_or; intros. right; reflexivity.
+  (* Inductive step *)
+  intros.
+  eapply startof_prefix in ENTRY; try eassumption.
+  eapply preservation_exec_prog in MDL; try (eassumption || apply loopnop_welltyped).
+  clear - PRE MDL. rename t1 into t. rename s into s0; rename s1 into s.
+  destruct_inv 64 PRE.
+  rename PRE into S0.
+  
+  repeat step; unfold arm8equiv in *; intros v SIG; specialize (S0 v SIG).
+  * rewrite N.eqb_eq in BC; subst; symmetry in Hsv.
+    destruct v; match goal with
+    | [ |- context[or (eq true true) _] ] => now left
+    | _ => right; repeat (rewrite update_updated || rewrite update_frame); try easy; 
+      match goal with | [ H: or (eq false true) _ |- _ ] => inversion H; [discriminate | easy]
+      end
+    end.
+  * destruct v; match goal with
+    | [ |- context[or (eq true true) _] ] => now left
+    | _ => right; repeat (rewrite update_updated || rewrite update_frame); try easy; 
+      match goal with | [ H: or (eq false true) _ |- _ ] => inversion H; [discriminate | easy]
+      end
+    end.
+Qed.
