Examples/p32_addloop.v
@@ -1,0 +1,45 @@
+Require Import NArith.
+Require Import ZArith.
+Require Import Picinae_pilbox32_interpreter.
+Require Import List.
+Import ListNotations.
+Open Scope N.
+
+Definition addloop_program := [
+  PIL_li 0 0; 
+  PIL_addi 1 1 1; 
+  PIL_subi 2 2 1; 
+  PIL_bne 0 2 (-8)%Z
+].
+
+Definition p32_addloop: addr -> N :=
+  p32_assemble'' 0x00 addloop_program.
+
+
+(*Compute p32_assemble 0x00 addloop_program.
+echo "     = [(0, 1); (1, 0); (2, 0); (3, 0); (4, 134); (
+        5, 36); (6, 0); (7, 0); (8, 8); (9, 41); (
+        10, 0); (11, 0); (12, 18); (13, 8); (
+        14, 255); (15, 255)]" | tr '(' '|' | tr -d '=[)];' | sed 's/,/ =>/g; s/|/\n|/g'
+
+*)
+Definition p32_addloop' : addr -> N :=
+fun a => match a with
+|0 => 1 (*   PIL_li 0 0;  *)
+|1 => 0
+|2 => 0
+|3 => 0
+|4 => 134 (*   PIL_addi 1 1 1;  *)
+|5 => 36
+|6 => 0
+|7 => 0
+|8 => 8 (*   PIL_subi 2 2 1;  *)
+|9 => 41
+|10 => 0
+|11 => 0
+|12 => 22 (*   PIL_subi 2 2 1;  *)
+|13 => 8
+|14 => 255
+|15 => 255
+|_ => 0
+end.
