Examples/p32_dynamicli.v
@@ -1,0 +1,42 @@
+Require Import NArith.
+Require Import ZArith.
+Require Import Picinae_pilbox32_interpreter.
+Require Import List.
+Require Import String.
+Import ListNotations.
+Open Scope N.
+
+Definition r0 := 0.
+Definition r1 := 1.
+Definition r5 := 5.
+
+
+Definition dynamic_li base_addr :=  [
+  PIL_li r0 0;
+  PIL_li r1 (assemble_insn (PIL_li r5 777));
+  PIL_st r1 r0 (base_addr + 3 * 4)
+  (* PIL_li r5 777;  <- dynamically written to memory section *)
+  ].
+
+Compute print_code (p32_assemble 0x00 (dynamic_li 0x00)) "p32_dynamicli"%string.
+
+Definition p32_dynamicli : addr -> N :=
+fun a => match a with
+  | 0 => 1
+  | 1 => 0
+  | 2 => 0
+  | 3 => 0
+  | 4 => 179
+  | 5 => 9
+  | 6 => 3
+  | 7 => 0
+  | 8 => 162
+  | 9 => 128
+  | 10 => 1
+  | 11 => 0
+  | _ => 0
+end.
+
+(* A more scalable way of creating the memory. *)
+Definition p32_dynamicli' := p32_assemble'' 0x00 (dynamic_li 0x00).
+
