Examples/p32_dynamicli_proof.v
@@ -1,0 +1,79 @@
+Require Import NArith.
+Require Import ZArith.
+Require Import Picinae_pilbox32_interpreter.
+Import PIL32Notations.
+Require Import p32_dynamicli.
+
+Definition dynamic_li_start : N :=  0.
+Definition dynamic_li_end   : N := 16.
+
+Section Invariants.
+  Variables inp1 inp2 : N.
+  Variable  s0 : store.
+  
+  Definition postcondition (s:store) := s R_R5 = Ⓓ(777).
+  Definition mem_unchanged (s:store) := s V_MEM32 = s0 V_MEM32 /\ s A_EXEC = s0 A_EXEC.
+  Definition invs (t:trace) : option Prop:=
+    match t with (Addr a, s) :: _ => match a with
+      | 0 => Some (mem_unchanged s)
+      | 16 => Some (postcondition s)
+      | _ => None end
+    | _ => None end.
+End Invariants.
+
+Definition dynamicli_exit (t:trace) :=
+  match t with (Addr a,_)::_ => match a with
+  | 16 => true
+  | _ => false
+  end | _ => false end.
+
+Definition exec_bits : addr -> N :=
+  fun a => match a with
+  | 0 | 4 | 8 | 12 => 1
+  | _ => 0 end.
+
+Theorem dynamicli_correctness:
+  forall s t s' x'
+         (ENTRY: startof t (x',s') = (Addr 0,s))
+         (MDL: models pil32typctx s)
+         (MEM: s V_MEM32 = Ⓜ p32_dynamicli')
+         (EXEC: s A_EXEC = Ⓜ exec_bits)
+,
+(* We define our program as p32_prog, a function that looks into
+   a given store's memory and page-execute permissions to determine
+   what the next instruction is.
+   Above we specified that the memory of the initial store is exactly
+   our program, which is held in bytes 0-12 with all other bytes 0.
+*)
+  satisfies_all p32_prog (invs s) dynamicli_exit ((x',s')::t).
+Proof.
+Local Ltac step := time pil32_step.
+intros. unfold satisfies_all.
+  apply prove_invs.
+  (* Base case: *)
+  simpl. rewrite ENTRY.
+  step. repeat (split; try assumption).
+
+  (* Inductive cases *)
+  intros.
+  (* somehow `startof_prefix` is bound to the wrong theorem here... 
+     In the strspn example the theorem is preferentially bound to
+     Picinae.Picinae_armv8_pcode.Theory_arm8.startof_prefix
+     rather than the alternative Picinae.Picinae_theory.startof_prefix.
+     Here it is the opposite, so we must specify the arch-specific version*)
+  eapply Picinae.Picinae_pilbox32.Theory_pil32.startof_prefix in ENTRY; try eassumption.
+  eapply preservation_exec_prog in MDL; try (eassumption || apply welltyped_p32prog).
+  clear - PRE MDL MEM EXEC. rename s into s0, t1 into t, s1 into s.
+
+  destruct_inv 32 PRE.
+  destruct PRE as [MEMSAME EXECSAME].
+  step.
+  step.
+  step.
+  (* Notice our address, 12, is exactly the location where we stored a 
+     value, 12443, in memory. 12433 corresponds exactly to`PIL_li r5 777,`
+     the instruction for loading the immediate 777 into register 5.
+  *)
+  step.
+  reflexivity.
+Qed.
