Picinae_pilbox32.v
@@ -1,0 +1,331 @@
+(* Picinae: Platform In Coq for INstruction Analysis of Executables       ZZM7DZ
+                                                                          $MNDM7
+   Copyright (c) 2023 Kevin W. Hamlen            ,,A??=P                 OMMNMZ+
+   The University of Texas at Dallas         =:$ZZ$+ZZI                  7MMZMZ7
+   Computer Science Department             Z$$ZM++O++                    7MMZZN+
+                                          ZZ$7Z.ZM~?                     7MZDNO$
+                                        ?Z8ZO7.OM=+?                     $OMO+Z+
+   Any use, commercial or otherwise       ?D=++M++ZMMNDNDZZ$$Z?           MM,IZ=
+   requires the express permission of        MZZZZZZ+...=.8NOZ8NZ$7       MM+$7M
+   the author.                                 ?NNMMM+.IZDMMMMZMD8O77     O7+MZ+
+                                                     MMM8MMMMMMMMMMM77   +MMMMZZ
+                                                     MMMMMMMMMMMZMDMD77$.ZMZMM78
+                                                      MMMMMMMMMMMMMMMMMMMZOMMM+Z
+   Instantiation of Picinae for PILbox32 ISA.          MMMMMMMMMMMMMMMMM^NZMMN+Z
+                                                        MMMMMMMMMMMMMMM/.$MZM8O+
+   To compile this module, first load and compile:       MMMMMMMMMMMMMM7..$MNDM+
+   * Picinae_core                                         MMDMMMMMMMMMZ7..$DM$77
+   * Picinae_theory                                        MMMMMMM+MMMZ7..7ZM~++
+   * Picinae_finterp                                        MMMMMMMMMMM7..ZNOOMZ
+   * Picinae_statics                                         MMMMMMMMMM$.$MOMO=7
+                                                              MDMMMMMMMO.7MDM7M+
+   Then compile this module with menu option                   ZMMMMMMMM.$MM8$MN
+   Compile->Compile_buffer.                                    $ZMMMMMMZ..MMMOMZ
+                                                                ?MMMMMM7..MNN7$M
+                                                                 ?MMMMMZ..MZM$ZZ
+                                                                  ?$MMMZ7.ZZM7DZ
+                                                                    7MMM$.7MDOD7
+                                                                     7MMM.7M77ZZ
+                                                                      $MM78ZDZ7Z
+                                                                        MM8D$7Z7
+                                                                        MM7O$$+Z
+                                                                         M 7N8ZD
+ *)
+
+Require Export Picinae_core.
+Require Export Picinae_theory.
+Require Export Picinae_statics.
+Require Export Picinae_finterp.
+Require Export Picinae_simplifier_v1_1.
+Require Import NArith.
+Require Import Program.Equality.
+Require Import Structures.Equalities.
+Open Scope N.
+
+(* Variables found in IL code lifted from ARM native code: *)
+Inductive pil32var :=
+  (* Main memory: 32 bit-width addresses, 2^32 bytes *)
+  | V_MEM32
+  (* 0-5, SP, LR = 32bit registers. *)
+  | R_R0 | R_R1 | R_R2 | R_R3 | R_R4 | R_R5
+  (* SP = stack pointer *)
+  | R_SP
+  (* LR = link register *)
+  | R_LR
+  (* PC = program counter *)
+  | R_PC
+  (* These meta-variables model page access permissions: *)
+  | A_READ | A_WRITE | A_EXEC.
+
+(* Create a UsualDecidableType module (which is an instance of Typ) to give as
+   input to the Architecture module, so that it understands how the variable
+   identifiers chosen above are syntactically written and how to decide whether
+   any two variable instances refer to the same variable. *)
+
+Module MiniPIL32VarEq <: MiniDecidableType.
+  Definition t := pil32var.
+  Definition eq_dec (v1 v2:pil32var) : {v1=v2}+{v1<>v2}.
+    decide equality; apply N.eq_dec.
+  Defined.  (* <-- This must be Defined (not Qed!) for finterp to work! *)
+  Arguments eq_dec v1 v2 : simpl never.
+End MiniPIL32VarEq.
+
+Module PIL32Arch <: Architecture.
+  Module Var := Make_UDT MiniPIL32VarEq.
+  Definition var := Var.t.
+  Definition store := var -> value.
+
+  Definition mem_bits := 8%positive.
+  Definition mem_readable s a := exists r, s A_READ = VaM r 32 /\ r a <> 0.
+  Definition mem_writable s a := exists w, s A_WRITE = VaM w 32 /\ w a <> 0.
+End PIL32Arch.
+
+(* Instantiate the Picinae modules with the arm identifiers above. *)
+Module IL_pil32 := PicinaeIL PIL32Arch.
+Export IL_pil32.
+Module Theory_pil32 := PicinaeTheory IL_pil32.
+Export Theory_pil32.
+Module Statics_pil32 := PicinaeStatics IL_pil32 Theory_pil32.
+Export Statics_pil32.
+Module FInterp_pil32 := PicinaeFInterp IL_pil32 Theory_pil32 Statics_pil32.
+Export FInterp_pil32.
+
+Module PSimpl_pil32 := Picinae_Simplifier_Base.
+Export PSimpl_pil32.
+Module PSimpl_pil32_v1_1 := Picinae_Simplifier_v1_1 IL_pil32 Theory_pil32 Statics_pil32 FInterp_pil32.
+Ltac PSimpl_pil32.PSimplifier ::= PSimpl_pil32_v1_1.PSimplifier.
+
+(* Introduce unique aliases for tactics in case user loads multiple architectures. *)
+Tactic Notation "pil32_psimpl" uconstr(e) "in" hyp(H) := psimpl_exp_hyp uconstr:(e) H.
+Tactic Notation "pil32_psimpl" uconstr(e) := psimpl_exp_goal uconstr:(e).
+Tactic Notation "pil32_psimpl" "in" hyp(H) := psimpl_all_hyp H.
+Tactic Notation "pil32_psimpl" := psimpl_all_goal.
+
+(* To use a different simplifier version (e.g., v1_0) put the following atop
+   your proof .v file:
+Require Import Picinae_simplifier_v1_0.
+Module PSimpl_pil32_v1_0 := Picinae_Simplifier_v1_0 IL_pil32 Statics_pil32 FInterp_pil32.
+Ltac PSimpl_pil32.PSimplifier ::= PSimpl_pil32_v1_0.PSimplifier.
+*)
+
+(* Declare the types (i.e., bitwidths) of all the CPU registers: *)
+Definition pil32typctx (id:var) : option typ :=
+  match id with
+  | V_MEM32 => Some (MemT 32)
+  | R_R0 | R_R1 | R_R2 | R_R3 | R_R4 | R_R5 => Some (NumT 32)
+  | R_SP | R_LR | R_PC => Some (NumT 32)
+  | A_READ | A_WRITE | A_EXEC => Some (MemT 32)
+end.
+
+(* Declare which context values are used to define store equivalence *)
+Definition pil32equivctx (id:var) : bool :=
+  match id with
+  | V_MEM32
+  | R_R0 | R_R1 | R_R2 | R_R3 | R_R4 | R_R5
+  | R_SP | R_LR => true
+  | _ => false
+  end.
+Definition pil32equiv (s1 s2:store) :=
+  forall (v:pil32var), pil32equivctx v = true -> s1 v = s2 v.
+Definition pil32equiv_or (s1 s2:store) (or_exception : pil32var -> bool) :=
+  forall (v:pil32var), pil32equivctx v = true -> or_exception v = true \/ s1 v = s2 v.
+Definition pil32_wtm {s v m w} := @models_wtm v pil32typctx s m w.
+Definition pil32_regsize {s v n w} := @models_regsize v pil32typctx s n w.
+
+
+
+(* TODO: how should we change the memory access machinery?
+         How does it work anyhoo? *)
+(* Simplify memory access propositions by observing that on arm, the only part
+   of the store that affects memory accessibility are the page-access bits
+   (A_READ and A_WRITE). *)
+
+Lemma memacc_read_frame:
+  forall s v u (NE: v <> A_READ),
+  MemAcc mem_readable (update s v u) = MemAcc mem_readable s.
+Proof.
+  intros. unfold MemAcc, mem_readable. rewrite update_frame. reflexivity.
+  apply not_eq_sym. exact NE.
+Qed.
+
+Lemma memacc_write_frame:
+  forall s v u (NE: v <> A_WRITE),
+  MemAcc mem_writable (update s v u) = MemAcc mem_writable s.
+Proof.
+  intros. unfold MemAcc, mem_writable. rewrite update_frame. reflexivity.
+  apply not_eq_sym. exact NE.
+Qed.
+
+Lemma memacc_read_updated:
+  forall s v u1 u2,
+  MemAcc mem_readable (update (update s v u2) A_READ u1) =
+  MemAcc mem_readable (update s A_READ u1).
+Proof.
+  intros. unfold MemAcc, mem_readable. rewrite !update_updated. reflexivity.
+Qed.
+
+Lemma memacc_write_updated:
+  forall s v u1 u2,
+  MemAcc mem_writable (update (update s v u2) A_WRITE u1) =
+  MemAcc mem_writable (update s A_WRITE u1).
+Proof.
+  intros. unfold MemAcc, mem_writable. rewrite !update_updated. reflexivity.
+Qed.
+
+(* Simplify arm memory access assertions produced by step_stmt. *)
+Ltac simpl_memaccs H :=
+  try lazymatch type of H with context [ MemAcc mem_writable ] =>
+    rewrite ?memacc_write_frame, ?memacc_write_updated in H by discriminate 1
+  end;
+  try lazymatch type of H with context [ MemAcc mem_readable ] =>
+    rewrite ?memacc_read_frame, ?memacc_read_updated in H by discriminate 1
+  end.
+
+(* The user can ignore all assigned values to specified variables by
+   redefining pil32_ignore.  Example:
+     Ltac pil32_ignore v ::= constr:(match v with R_EAX => true | _ => false end).
+ *)
+Ltac pil32_ignore v := constr:(false).
+Ltac pil32_abstract_vars H :=
+  repeat match type of H with context [ update ?s ?v ?u ] =>
+    let b := ltac:(pil32_ignore v) in
+    lazymatch eval cbv in b with true =>
+      lazymatch u with
+      | VaN ?n ?w =>
+          tryif is_var n then fail else
+          let tmp := fresh "n" in
+          pose (tmp := n);
+          change (update s v (VaN n w)) with (update s v (VaN tmp w)) in H;
+          clearbody tmp
+      | VaM ?m ?w =>
+          tryif is_var m then fail else
+          let tmp := fresh "m" in
+          pose (tmp := m);
+          change (update s v (VaM m w)) with (update s v (VaM tmp w)) in H;
+          clearbody tmp
+      end
+    | _ => fail
+    end
+  end.
+
+(* Symbolically evaluate an arm machine instruction for one step, and simplify
+   the resulting Coq expressions. *)
+Ltac pil32_step_and_simplify XS :=
+  step_stmt XS;
+  pil32_abstract_vars XS;
+  psimpl_vals_hyp XS;
+  simpl_memaccs XS;
+  destruct_memaccs XS.
+
+(* Introduce automated machinery for verifying an pil32 machine code subroutine
+   (or collection of subroutines) by (1) defining a set of Floyd-Hoare
+   invariants (including pre- and post-conditions) and (2) proving that
+   symbolically executing the program starting at any invariant point in a
+   state that satisfies the program until the next invariant point always
+   yields a state that satisfies the reached invariant.  This proves partial
+   correctness of the subroutine.
+
+   In order for this methodology to prove that a post-condition holds at
+   subroutine exit, we must attach one of these invariants (the post-condition)
+   to the return address of the subroutine.  This is a somewhat delicate
+   process, since unlike most other code addresses, the exact value of the
+   return address is an unknown (defined by the caller).  We therefore adopt
+   the convention that subroutines "exit" whenever control flows to an address
+   for which no IL code is defined at that address.  This allows proving
+   correctness of a subroutine by lifting only the subroutine to IL code (or
+   using the pmono theorems from Picinae_theory to isolate only the subroutine
+   from a larger program), leaving the non-subroutine code undefined (None). *)
+
+(* Some versions of Coq check injection-heavy proofs very slowly (at Qed).
+   This slow-down can be avoided by sequestering prevalent injections into
+   lemmas, as we do here. *)
+Remark inj_prog_stmt: forall (sz1 sz2: N) (q1 q2: stmt),
+                      Some (sz1,q1) = Some (sz2,q2) -> sz1=sz2 /\ q1=q2.
+Proof. injection 1 as. split; assumption. Qed.
+
+(* Simplify (exitof a x) without expanding a. *)
+Remark exitof_none a: exitof a None = Addr a. Proof eq_refl.
+Remark exitof_some a x: exitof a (Some x) = x. Proof eq_refl.
+
+
+(* If asked to step the computation when we're already at an invariant point,
+   just make the proof goal be the invariant. *)
+Ltac pil32_invhere :=
+  eapply nextinv_here; [ reflexivity | hnf; psimpl_vals_goal ].
+
+(* Rewrite facts about the store's memory to enable dynamically interpreted
+   programs (programs in which instructions are decoded from the bytes stored
+   in memory.)  *)
+Ltac pil32_prog_simpl :=
+  unfold effinv, effinv';
+  repeat match goal with
+  | [ H: store |- context[?p ?H _]] => unfold p
+  | [ H: eq ?SM (VaM _ _) |- context[match ?SM with _ => _ end]] => rewrite H
+  | [ H2: eq ?SM2 (VaM _ _) ,
+      H1: eq ?SM1 ?SM2 |- context[match ?SM1 with _ => _ end]] => rewrite <-H1 in H2; rewrite H2
+  end.
+
+(* If we're not at an invariant, symbolically interpret the program for one
+   machine language instruction.  (The user can use "do" to step through many
+   instructions, but often it is wiser to pause and do some manual
+   simplification of the state at various points.) *)
+Ltac pil32_invseek :=
+  eapply NIStep; [pil32_prog_simpl; reflexivity|pil32_prog_simpl; reflexivity|];
+  let s := fresh "s" in let x := fresh "x" in let XS := fresh "XS" in
+  intros s x XS;
+  pil32_step_and_simplify XS;
+  repeat lazymatch type of XS with
+         | s=_ /\ x=_ => destruct XS; subst s x
+         | exec_stmt _ (if ?c then _ else _) _ _ =>
+             let BC := fresh "BC" in destruct c eqn:BC;
+             pil32_step_and_simplify XS
+         | exec_stmt _ (N.iter _ _ _) _ _ => fail
+         | _ => pil32_step_and_simplify XS
+         end;
+  try match goal with |- nextinv _ _ _ _ (_ :: ?xs :: ?t) =>
+    let t' := fresh t in generalize (xs::t); intro t'; clear t; rename t' into t
+  end;
+  repeat match goal with [ u:value |- _ ] => clear u
+                       | [ n:N |- _ ] => clear n
+                       | [ m:addr->N |- _ ] => clear m end;
+  try lazymatch goal with |- context [ exitof (N.add ?m ?n) ] => simpl (N.add m n) end;
+  try first [ rewrite exitof_none | rewrite exitof_some ].
+
+(* Clear any stale memory-access hypotheses (arising from previous computation
+   steps) and either step to the next machine instruction (if we're not at an
+   invariant) or produce an invariant as a proof goal. *)
+Ltac pil32_step :=
+  repeat match goal with [ H: MemAcc _ _ _ _ _ |- _ ] => clear H end;
+  first [ pil32_invseek; try pil32_invhere | pil32_invhere ].
+
+
+Declare Scope pil32_scope.
+Delimit Scope pil32_scope with pil32.
+Bind Scope pil32_scope with stmt exp typ trace.
+Open Scope pil32_scope.
+Notation " s1 $; s2 " := (Seq s1 s2) (at level 75, right associativity) : pil32_scope.
+
+Module PIL32Notations.
+
+Notation "Ⓜ m" := (VaM m 32) (at level 20, format "'Ⓜ' m"). (* memory value *)
+Notation "ⓑ u" := (VaN u 1) (at level 20, format "'ⓑ' u"). (* bit value *)
+Notation "Ⓑ u" := (VaN u 8) (at level 20, format "'Ⓑ' u"). (* byte value *)
+Notation "Ⓦ u" := (VaN u 16) (at level 20, format "'Ⓦ' u"). (* word value *)
+Notation "Ⓓ u" := (VaN u 32) (at level 20, format "'Ⓓ' u"). (* dword value *)
+Notation "m Ⓑ[ a  ]" := (getmem 32 LittleE 1 m a) (at level 30) : pil32_scope. (* read byte from memory *)
+Notation "m Ⓦ[ a  ]" := (getmem 32 LittleE 2 m a) (at level 30) : pil32_scope. (* read word from memory *)
+Notation "m Ⓓ[ a  ]" := (getmem 32 LittleE 4 m a) (at level 30) : pil32_scope. (* read dword from memory *)
+Notation "m [Ⓑ  a := v  ]" := (setmem 32 LittleE 1 m a v) (at level 50, left associativity) : pil32_scope. (* write byte to memory *)
+Notation "m [Ⓦ  a := v  ]" := (setmem 32 LittleE 2 m a v) (at level 50, left associativity) : pil32_scope. (* write word to memory *)
+Notation "m [Ⓓ  a := v  ]" := (setmem 32 LittleE 4 m a v) (at level 50, left associativity) : pil32_scope. (* write dword to memory *)
+Notation "x ⊕ y" := ((x+y) mod 2^32) (at level 50, left associativity). (* modular addition *)
+Notation "x ⊖ y" := (msub 32 x y) (at level 50, left associativity). (* modular subtraction *)
+Notation "x ⊗ y" := ((x*y) mod 2^32) (at level 40, left associativity). (* modular multiplication *)
+Notation "x << y" := (N.shiftl x y) (at level 55, left associativity). (* logical shift-left *)
+Notation "x >> y" := (N.shiftr x y) (at level 55, left associativity). (* logical shift-right *)
+Notation "x >>> y" := (ashiftr 32 x y) (at level 55, left associativity). (* arithmetic shift-right *)
+Notation "x .& y" := (N.land x y) (at level 56, left associativity). (* logical and *)
+Notation "x .^ y" := (N.lxor x y) (at level 57, left associativity). (* logical xor *)
+Notation "x .| y" := (N.lor x y) (at level 58, left associativity). (* logical or *)
+
+End PIL32Notations.
