Picinae_pilbox32_interpreter.v
@@ -1,0 +1,789 @@
+Require Export Picinae_pilbox32.
+
+Require Export Picinae_core.
+Require Export Picinae_theory.
+Require Export Picinae_statics.
+Require Export Picinae_finterp.
+Require Export Picinae_simplifier_v1_1.
+Require Import NArith.
+Require Import ZArith.
+Require Import Program.Equality.
+Require Import Structures.Equalities.
+Require Import Lia.
+Require Import FunctionalExtensionality.
+Require Import String.
+Require Import List.
+Open Scope N.
+
+Import PIL32Notations.
+
+Inductive p32_asm :=
+(* Arithmetic *)
+| PIL_add (rd rs1 rs2:N)
+| PIL_sub (rd rs1 rs2:N)
+| PIL_addi (rd rs1:N) (i:N)
+| PIL_subi (rd rs1:N) (i:N)
+| PIL_li (rd:N) (i:N)
+(* Logical *)
+| PIL_and (rd rs1 rs2:N)
+| PIL_or  (rd rs1 rs2:N)
+| PIL_xor (rd rs1 rs2:N)
+| PIL_not (rd rs1:N)
+(* Control Flow *)
+| PIL_beq (rs1 rs2:N) (si:Z)
+| PIL_blt (rs1 rs2:N) (si:Z)
+| PIL_bne (rs1 rs2:N) (si:Z)
+| PIL_bl (si:Z)
+| PIL_jl (i:N)
+| PIL_jmp (i:N)
+| PIL_jmpr (rs1:N)
+(* Memory Access *)
+(* address to store/load is *rd + i *)
+| PIL_ld (rd rs:N) (i:N)
+| PIL_st (rs rd:N) (i:N)
+(* Invalid *)
+| PIL_InvalidI.
+
+Definition p32_decode_binop_reg op rd rs1 rs2 :=
+  match op with
+  | 1 => PIL_add rd rs1 rs2
+  | 2 => PIL_sub rd rs1 rs2
+  | 5 => PIL_and rd rs1 rs2
+  | 6 => PIL_or  rd rs1 rs2
+  | 7 => PIL_xor rd rs1 rs2
+  | 8 => PIL_not rd rs1
+  | _ => PIL_InvalidI
+  end.
+ 
+Definition p32_decode_binop_imm op rd rs1 i :=
+  match op with
+  | 3 => PIL_addi rd rs1 i
+  | 4 => PIL_subi rd rs1 i
+  | _ => PIL_InvalidI
+  end.
+
+Definition p32_decode_cf_simm op rs1 rs2 (si:Z) :=
+  match op with
+  | 9  => PIL_beq rs1 rs2 si
+  | 10 => PIL_blt rs1 rs2 si
+  | 11 => PIL_bne rs1 rs2 si
+  | _ => PIL_InvalidI
+  end.
+
+Definition p32_decode_memacc op rs rd i :=
+  match op with
+  | 16 => PIL_ld rs rd i
+  | 17 => PIL_st rs rd i
+  | _ => PIL_InvalidI
+  end.
+
+Definition p32_decode_simm op si :=
+  match op with
+  | 12 => PIL_bl si
+  | _ => PIL_InvalidI
+  end.
+
+Definition p32_decode_imm op i :=
+  match op with
+  | 13 => PIL_jl i
+  | 14 => PIL_jmp i
+  | _ => PIL_InvalidI
+  end.
+
+Definition p32_decode_reg op r :=
+  match op with
+  | 15 => PIL_jmpr r
+  | _  => PIL_InvalidI
+  end.
+
+
+(* bit 0 - if set then load immediate; else the following
+   bits 1-6 : opcode
+   bits 7-9 : usually reg
+   bits 10-12 : usually reg
+   bits 13-15 : usually reg / imm
+*)
+Definition p32_decode_op op n : p32_asm:=
+  if N.testbit op 0 then PIL_li (xnbits n 1 3) (xnbits n 4 28) else
+  match op >> 1 with
+  | 1 | 2 | 5 | 6 | 7 | 8 => p32_decode_binop_reg (op >> 1) (xnbits n 7 3) (xnbits n 10 3) (xnbits n 13 3)
+  | 3 | 4 => p32_decode_binop_imm (op >> 1) (xnbits n 7 3) (xnbits n 10 3) (xnbits n 13 19)
+  | 9 | 10 | 11 => p32_decode_cf_simm (op >> 1) (xnbits n 7 3) (xnbits n 10 3) (toZ 19 (xnbits n 13 19))
+  | 12 => p32_decode_simm (op >> 1) (toZ 25 (xnbits n 7 25))
+  | 13 | 14 => p32_decode_imm (op >> 1) (xnbits n 7 25)
+  | 15 => p32_decode_reg (op >> 1) (xnbits n 7 3)
+  | 16 | 17 => p32_decode_memacc (op >> 1) (xnbits n 7 3) (xnbits n 10 3) (xnbits n 13 19)
+  | _ => PIL_InvalidI
+  end.
+
+Definition p32_decode n : p32_asm :=
+  p32_decode_op (N.land n (N.ones 6)) n.
+
+Definition p32_varid (n:N) :=
+  match n with
+  | 0 => R_R0 | 1 => R_R1 | 2 => R_R2 | 3 => R_R3
+  | 4 => R_R4 | 5 => R_R5 | 6 => R_SP | 7 => R_LR 
+  (* What to do for this invalid case? *)
+  | _ => R_PC
+  end.
+
+Definition p32var (n:N) := Var (p32_varid n).
+Arguments p32var / !n.
+Definition TRUE_EXP := Word 1 1.
+Definition p32mov n e := Move (p32_varid n) e.
+Definition p32branch e a (off:Z) :=
+    If e (Jmp (Word ((Z.to_N (Z.of_N a + off)) mod 2^32) 32)) Nop.
+(*  let new_pc_exp := (BinOp (match off with | Z.neg _ => OP_MINUS | _ => OP_PLUS end) (Word a 32) (Word (ofZ 32 (Z.abs off)) 32)) in
+  If e (Jmp (BinOp OP_PLUS new_pc_exp (Word 4 32))) Nop.
+*)
+
+Definition p322il a p32i :=
+  match p32i with
+  | PIL_InvalidI => Exn 2
+
+  (* Integer Computational Instructions *)
+  | PIL_add rd rs1 rs2 => p32mov rd (BinOp OP_PLUS (p32var rs1) (p32var rs2))
+  | PIL_sub rd rs1 rs2 => p32mov rd (BinOp OP_MINUS (p32var rs1) (p32var rs2))
+  | PIL_addi rd rs1 imm => p32mov rd (BinOp OP_PLUS (p32var rs1) (Word imm 32))
+  | PIL_subi rd rs1 imm => p32mov rd (BinOp OP_MINUS (p32var rs1) (Word imm 32))
+  | PIL_li rd imm =>  p32mov rd (Word imm 32)
+  | PIL_and rd rs1 rs2 => p32mov rd (BinOp OP_AND (p32var rs1) (p32var rs2))
+  | PIL_or  rd rs1 rs2 => p32mov rd (BinOp OP_OR  (p32var rs1) (p32var rs2))
+  | PIL_xor rd rs1 rs2 => p32mov rd (BinOp OP_XOR (p32var rs1) (p32var rs2))
+  | PIL_not rd rs1 => p32mov rd (UnOp OP_NEG (p32var rs1))
+
+
+  (* Conditional Transfer Instructions *)
+  | PIL_beq rs1 rs2 simm => p32branch (BinOp OP_EQ  (p32var rs1) (p32var rs2)) a simm
+  | PIL_blt rs1 rs2 simm => p32branch (BinOp OP_LT  (p32var rs1) (p32var rs2)) a simm
+  | PIL_bne rs1 rs2 simm => p32branch (BinOp OP_NEQ (p32var rs1) (p32var rs2)) a simm
+
+    (* Unconditional jumps *)
+  | PIL_bl simm => Seq (Move R_LR (Word ((a+4) mod 2^32) 32)) (p32branch TRUE_EXP a simm)
+  | PIL_jl imm => Seq (Move R_LR (Word ((a+4) mod 2^32) 32)) (Jmp (Word imm 32))
+  | PIL_jmp imm => Jmp (Word imm 32)
+  | PIL_jmpr rs => Jmp (p32var rs)
+
+  (* Load and Store Instructions *)
+  | PIL_ld rd rs imm => p32mov rd (Load (Var V_MEM32) (BinOp OP_PLUS (p32var rs) (Word imm 32)) LittleE 4)
+  | PIL_st rs rd imm => Move V_MEM32 (Store (Var V_MEM32) (BinOp OP_PLUS (p32var rd) (Word imm 32)) (p32var rs) LittleE 4)
+
+  end.
+  
+
+(* Here we enforce that all instruction fetches must start at a word
+   aligned boundary. When we have a variable-length interpreter we
+   will need to relax this constraint and introduce another layer of
+   complexity.
+*)
+Definition p32_stmt m a :=
+  p322il a match a mod 4 with 0 => p32_decode (getmem 32 LittleE 4 m a) | _ => PIL_InvalidI end.
+
+Definition p32_prog : program :=
+  fun s a => match s V_MEM32, s A_EXEC with
+             | VaM m _, VaM e _ => match e a with
+                                   | N0 => None
+                                   | _ => Some (4, p32_stmt m a)
+                                   end
+             | _, _ => None
+             end.
+
+
+Lemma hastyp_p32mov:
+  forall c0 c n e (TS: hastyp_stmt c0 c (Move (p32_varid n) e) c),
+  hastyp_stmt c0 c (p32mov n e) c.
+Proof.
+  intros. unfold p32mov, p32_varid in *. exact TS.
+Qed.
+
+Lemma hastyp_pthirtytwomov:
+  forall n e (TE: hastyp_exp pil32typctx e (NumT 32)),
+  hastyp_stmt pil32typctx pil32typctx (Move (p32_varid n) e) pil32typctx.
+Proof.
+  intros. erewrite store_upd_eq at 3.
+    eapply TMove.
+      right. destruct n as [|n]. reflexivity. repeat first [ reflexivity | destruct n as [n|n|] ].
+      exact TE.
+      reflexivity.
+    destruct n as [|n]. reflexivity. repeat first [ reflexivity | destruct n as [n|n|] ].
+Qed.
+
+Lemma hastyp_p32store:
+  forall e (TE: hastyp_exp pil32typctx e (MemT 32)),
+  hastyp_stmt pil32typctx pil32typctx (Move V_MEM32 e) pil32typctx.
+Proof.
+  intros. erewrite store_upd_eq at 3.
+    eapply TMove.
+      right. reflexivity.
+      exact TE.
+      reflexivity.
+    reflexivity.
+Qed.
+
+Lemma p32varid_numt32:
+  forall n, pil32typctx (p32_varid n) = Some (NumT 32).
+Proof.
+  intro. unfold p32_varid.
+  destruct n as [|n]; try reflexivity. unfold pil32typctx.
+  (* Why doesn't this work: repeat (reflexivity || destruct n as [n]). *)
+  destruct n; try destruct n; try destruct n.
+  all: reflexivity.
+Qed.
+
+Lemma hastyp_p32var:
+  forall n, hastyp_exp pil32typctx (p32var n) (NumT 32).
+Proof.
+  intro. unfold p32var, p32_varid.
+  apply TVar. destruct n as [|n]; try reflexivity. unfold pil32typctx.
+  (* Why doesn't this work: repeat (reflexivity || destruct n as [n]). *)
+  destruct n; try destruct n; try destruct n.
+  all: reflexivity.
+Qed.
+
+
+Theorem varupdate_nop:
+  forall n, pil32typctx[p32_varid n := Some (NumT 32)] = pil32typctx.
+Proof.
+  unfold update, pil32typctx; intros. extensionality a.
+  assert (H: forall v n, v = p32_varid n -> v <> V_MEM32 /\ v <> A_READ /\ v <> A_WRITE /\ v <> A_EXEC).
+    clear n a; unfold p32_varid; intros. subst. repeat split.
+    1-4: destruct n as [|p];[
+        intros; discriminate
+      | repeat (intros;discriminate || destruct p as [p|p|])].
+  destruct (a==p32_varid n). 
+    specialize (H a n e). destruct H as [H1 [H2 [H3 h4]]]. subst a. destruct (p32_varid n); easy.
+    destruct a; try reflexivity.
+Qed.
+
+Theorem regupdate_nop:
+  forall r, match r with 
+  | V_MEM32 | A_READ | A_WRITE | A_EXEC => True
+  | _ => pil32typctx[r := Some (NumT 32)] = pil32typctx
+  end.
+Proof.
+  intros; unfold update; destruct r; try apply I; extensionality a;
+    destruct (a == _); subst; reflexivity.
+Qed.
+
+Theorem hastyp_varupdate:
+  forall n, pil32typctx ⊆ pil32typctx[p32_varid n := Some (NumT 32)].
+Proof.
+  unfold pfsub, update. intros.
+    destruct (x == p32_varid n); subst.
+      now rewrite p32varid_numt32 in H.
+      assumption.
+Qed.
+
+
+Theorem hastyp_word:
+  forall c n pl pr, pl <= pr -> hastyp_exp c (Word (n mod 2 ^ pl) pr) (NumT pr).
+Proof. 
+  intros. econstructor. apply N.lt_le_trans with (m:=2^pl).
+    apply mp2_mod_lt.
+    apply N.pow_le_mono_r; lia.
+Qed.
+
+
+Ltac Zify.zify_post_hook ::= Z.div_mod_to_equations.
+
+Theorem welltyped_p322il:
+  forall a n, hastyp_stmt pil32typctx pil32typctx (p322il a (p32_decode n)) pil32typctx.
+Proof.
+  intros.
+  unfold p32_decode, p32_decode_op, p32_decode_binop_reg, p32_decode_binop_imm,
+    p32_decode_cf_simm, p32_decode_memacc, p32_decode_simm, p32_decode_imm, p32_decode_reg.
+
+  repeat match goal with |- context [ match ?x with _ => _ end ] =>
+    let op := fresh "op" in
+    generalize x; intro op;
+    first [ destruct op as [|op] | destruct op as [op|op|] ];
+    try apply TExn
+  end.
+
+  all: try solve [ do 2 repeat first
+  [ reflexivity
+  | discriminate 1
+  | apply hastyp_p32mov
+  | apply hastyp_p32mov
+  | apply hastyp_p32var
+  | apply hastyp_p32store
+  | apply TBinOp with (w:=32)
+  | apply hastyp_varupdate
+  | eapply N.lt_le_trans; [apply xnbits_bound + apply xbits_bound|]
+  | apply ofZ_bound
+  | apply N.mod_lt
+  | econstructor ] ].
+
+  Ltac destruct_var n b tac:=
+    destruct (xnbits n b 3) as [|p]; repeat (tac || destruct p as [p|p|]).
+  Ltac duh := try right; try ( (apply hastyp_word; lia) || (apply hastyp_varupdate) ); try now rewrite p32varid_numt32;
+    try (apply TBinOp with (w:=32); apply hastyp_p32var || apply hastyp_word; try lia).
+  Ltac econs_duh := econstructor; duh.
+  all: econs_duh; repeat first 
+    [ apply TBinOp with (w:=32)
+    | apply hastyp_p32var 
+    | apply hastyp_word
+    | rewrite varupdate_nop
+    |   match goal with
+        | [|-context[update _ ?R (Some (NumT 32))]] 
+            => rewrite (regupdate_nop R) 
+        end
+    | lia
+    | solve apply pfsub_refl
+    | econs_duh]. 
+  all: try rewrite varupdate_nop; try apply pfsub_refl; try lia.
+  Unshelve. all:exact 0.
+Qed.
+
+Theorem welltyped_p32prog:
+  welltyped_prog pil32typctx p32_prog.
+Proof.
+  intros s a. unfold p32_prog.
+  destruct (s V_MEM32), (s A_EXEC); try exact I.
+  destruct (m0 a).
+    exact I.
+    exists pil32typctx. unfold p32_stmt. destruct (a mod 4).
+      apply welltyped_p322il.
+      apply TExn. reflexivity.
+Qed.
+
+
+(* Create some automated machinery for simplifying symbolic expressions. *)
+
+Lemma memacc_read_frame:
+  forall s v u (NE: v <> A_READ),
+  MemAcc mem_readable (update s v u) = MemAcc mem_readable s.
+Proof.
+  intros. unfold MemAcc, mem_readable. rewrite update_frame. reflexivity.
+  apply not_eq_sym. exact NE.
+Qed.
+
+Lemma memacc_write_frame:
+  forall s v u (NE: v <> A_WRITE),
+  MemAcc mem_writable (update s v u) = MemAcc mem_writable s.
+Proof.
+  intros. unfold MemAcc, mem_writable. rewrite update_frame. reflexivity.
+  apply not_eq_sym. exact NE.
+Qed.
+
+Lemma memacc_read_updated:
+  forall s v u1 u2,
+  MemAcc mem_readable (update (update s v u2) A_READ u1) =
+  MemAcc mem_readable (update s A_READ u1).
+Proof.
+  intros. unfold MemAcc, mem_readable. rewrite !update_updated. reflexivity.
+Qed.
+
+Lemma memacc_write_updated:
+  forall s v u1 u2,
+  MemAcc mem_writable (update (update s v u2) A_WRITE u1) =
+  MemAcc mem_writable (update s A_WRITE u1).
+Proof.
+  intros. unfold MemAcc, mem_writable. rewrite !update_updated. reflexivity.
+Qed.
+
+(* Introduce automated machinery for verifying a RISC-V machine code subroutine
+   (or collection of subroutines) by (1) defining a set of Floyd-Hoare
+   invariants (including pre- and post-conditions) and (2) proving that
+   symbolically executing the program starting at any invariant point in a
+   state that satisfies the program until the next invariant point always
+   yields a state that satisfies the reached invariant.  This proves partial
+   correctness of the subroutine.
+
+   In order for this methodology to prove that a post-condition holds at
+   subroutine exit, we must attach one of these invariants (the post-condition)
+   to the return address of the subroutine.  This is a somewhat delicate
+   process, since unlike most other code addresses, the exact value of the
+   return address is an unknown (defined by the caller).  We therefore adopt
+   the convention that subroutines "exit" whenever control flows to an address
+   for which no IL code is defined at that address.  This allows proving
+   correctness of a subroutine by lifting only the subroutine to IL code (or
+   using the pmono theorems from Picinae_theory to isolate only the subroutine
+   from a larger program), leaving the non-subroutine code undefined (None). *)
+
+(* Simplify memory access assertions produced by step_stmt. *)
+Ltac simpl_memaccs H :=
+  try lazymatch type of H with context [ MemAcc mem_writable ] =>
+    rewrite ?memacc_write_frame, ?memacc_write_updated in H by discriminate 1
+  end;
+  try lazymatch type of H with context [ MemAcc mem_readable ] =>
+    rewrite ?memacc_read_frame, ?memacc_read_updated in H by discriminate 1
+  end.
+
+(* Symbolically evaluate a RISC-V machine instruction for one step. *)
+Ltac p32_step_and_simplify XS :=
+  step_stmt XS;
+  psimpl_vals_hyp XS;
+  simpl_memaccs XS;
+  destruct_memaccs XS.
+
+(* Some versions of Coq check injection-heavy proofs very slowly (at Qed).  This slow-down can
+   be avoided by sequestering prevalent injections into lemmas, as we do here. *)
+Remark inj_prog_stmt: forall (sz1 sz2: N) (q1 q2: stmt),
+                      Some (sz1,q1) = Some (sz2,q2) -> sz1=sz2 /\ q1=q2.
+Proof. injection 1 as. split; assumption. Qed.
+
+(* Simplify (exitof a x) without expanding a. *)
+Remark exitof_none a: exitof a None = Addr a. Proof eq_refl.
+Remark exitof_some a x: exitof a (Some x) = x. Proof eq_refl.
+
+(* If asked to step the computation when we're already at an invariant point,
+   just make the proof goal be the invariant. *)
+Ltac p32_invhere :=
+  eapply nextinv_here; [ reflexivity | red; psimpl_vals_goal ].
+
+(* If we're not at an invariant, symbolically interpret the program for one
+   machine language instruction.  (The user can use "do" to step through many
+   instructions, but often it is wiser to pause and do some manual
+   simplification of the state at various points.) *)
+Ltac p32_invseek :=
+  eapply NIStep; [reflexivity|reflexivity|];
+  let s := fresh "s" in let x := fresh "x" in let XS := fresh "XS" in
+  intros s x XS;
+  p32_step_and_simplify XS;
+  repeat lazymatch type of XS with
+         | s=_ /\ x=_ => destruct XS; subst s x
+         | exec_stmt _ (if ?c then _ else _) _ _ =>
+             let BC := fresh "BC" in destruct c eqn:BC;
+             p32_step_and_simplify XS
+         | exec_stmt _ (N.iter _ _ _) _ _ => fail
+         | _ => p32_step_and_simplify XS
+         end;
+  try match goal with |- nextinv _ _ _ _ (_ :: ?xs :: ?t) =>
+    let t' := fresh t in generalize (xs::t); intro t'; clear t; rename t' into t
+  end;
+  repeat match goal with [ u:value |- _ ] => clear u
+                       | [ n:N |- _ ] => clear n
+                       | [ m:addr->N |- _ ] => clear m end;
+  try lazymatch goal with |- context [ exitof (N.add ?m ?n) ] => simpl (N.add m n) end;
+  try first [ rewrite exitof_none | rewrite exitof_some ].
+
+(* Clear any stale memory-access hypotheses (arising from previous computation
+   steps) and either step to the next machine instruction (if we're not at an
+   invariant) or produce an invariant as a proof goal. *)
+Ltac p32_step :=
+  repeat match goal with [ H: MemAcc _ _ _ _ _ |- _ ] => clear H end;
+  first [ p32_invseek; try p32_invhere | p32_invhere ].
+
+
+(* Assembler section *)
+Definition assemble_insn_op (insn:p32_asm) : N :=
+  match insn with
+  | PIL_add rd rs1 rs2 => 1 << 1
+  | PIL_sub rd rs1 rs2 => 2 << 1
+  | PIL_addi rd rs1 i => 3 << 1
+  | PIL_subi rd rs1 i => 4 << 1
+  | PIL_and rd rs1 rs2 => 5 << 1
+  | PIL_or  rd rs1 rs2 => 6 << 1
+  | PIL_xor rd rs1 rs2 => 7 << 1
+  | PIL_not rd rs1 => 8 << 1
+  | PIL_beq rs1 rs2 si => 9 << 1
+  | PIL_blt rs1 rs2 si => 10 << 1
+  | PIL_bne rs1 rs2 si => 11 << 1
+  | PIL_bl si => 12 << 1
+  | PIL_jl i => 13 << 1
+  | PIL_jmp i => 14 << 1
+  | PIL_jmpr rs1 => 15 << 1
+  | PIL_ld rd rs i => 16 << 1
+  | PIL_st rs rd i => 17 << 1
+  | PIL_li rd i => 1
+  | PIL_InvalidI => 0
+  end.
+
+(* Definition p32_varid (n:N) :=
+  match n with
+  | 0 => R_R0 | 1 => R_R1 | 2 => R_R2 | 3 => R_R3
+  | 4 => R_R4 | 5 => R_R5 | 6 => R_SP | 7 => R_LR 
+  (* What to do for this invalid case? *)
+  | _ => R_PC
+  end.
+Definition assemble_reg (r:p32var) : option N :=
+  match r with
+  | R_R0 => 0 *)
+  
+Definition p32_decode_op_cp op n : p32_asm:=
+  if N.testbit op 0 then PIL_li (xnbits n 1 3) (xnbits n 4 28) else
+  match op >> 1 with
+  | 1 | 2 | 5 | 6 | 7 | 8 => p32_decode_binop_reg (op >> 1) (xnbits n 7 3) (xnbits n 10 3) (xnbits n 13 3)
+  | 3 | 4 => p32_decode_binop_imm (op >> 1) (xnbits n 7 3) (xnbits n 10 3) (xnbits n 13 19)
+  | 9 | 10 | 11 => p32_decode_cf_simm (op >> 1) (xnbits n 7 3) (xnbits n 10 3) (toZ 19 (xnbits n 13 19))
+  | 12 => p32_decode_simm (op >> 1) (toZ 25 (xnbits n 7 25))
+  | 13 | 14 => p32_decode_imm (op >> 1) (xnbits n 7 25)
+  | 15 => p32_decode_reg (op >> 1) (xnbits n 7 3)
+  | 16 | 17 => p32_decode_memacc (op >> 1) (xnbits n 7 3) (xnbits n 10 3) (xnbits n 13 19)
+  | _ => PIL_InvalidI
+  end.
+
+Definition assemble_insn (insn:p32_asm) : N :=
+  match insn with
+  | PIL_add rd rs1 rs2
+  | PIL_sub rd rs1 rs2
+  | PIL_and rd rs1 rs2
+  | PIL_or  rd rs1 rs2
+  | PIL_xor rd rs1 rs2 
+      => (assemble_insn_op insn) .| ( rd << 7) .| ( rs1 << 10) .| ( rs2 << 13)
+  | PIL_addi rd rs1 i
+  | PIL_subi rd rs1 i
+      => (assemble_insn_op insn) .| ( rd << 7) .| ( rs1 << 10) .| (i  << 13)
+  | PIL_not rd rs1
+      => (assemble_insn_op insn) .| ( rd << 7) .| ( rs1 << 10)
+  | PIL_beq rs1 rs2 si
+  | PIL_blt rs1 rs2 si
+  | PIL_bne rs1 rs2 si
+      => (assemble_insn_op insn) .| ( rs1 << 7) .| ( rs2 << 10) .| ((ofZ (32-13) si) << 13)
+  | PIL_bl si
+        => (assemble_insn_op insn) .| ((ofZ (32-7) si) << 7)
+  | PIL_jl i
+  | PIL_jmp i
+        => (assemble_insn_op insn) .| (i << 7)
+  | PIL_jmpr rs1
+        => (assemble_insn_op insn) .| ( rs1 << 7)
+  | PIL_ld r1 r2 i
+  | PIL_st r1 r2 i
+        => (assemble_insn_op insn) .| ( r1 << 7) .| ( r2 << 10) .| (i << 13)
+  | PIL_li rd i
+        => (assemble_insn_op insn) .| ( rd << 1) .| (i << 4)
+  | PIL_InvalidI => 0
+  end.
+
+Definition welltyped_p32_asm (insn:p32_asm) : Prop :=
+  match insn with
+  | PIL_add rd rs1 rs2
+  | PIL_sub rd rs1 rs2
+  | PIL_and rd rs1 rs2
+  | PIL_or  rd rs1 rs2
+  | PIL_xor rd rs1 rs2 
+      => rd < 8 /\ rs1 < 8 /\ rs2 < 8
+  | PIL_addi rd rs1 i
+  | PIL_subi rd rs1 i
+      => rd < 8 /\ rs1 < 8 /\ i < 2^(32-13)
+  | PIL_not rd rs1
+      => rd < 8 /\ rs1 < 8
+  | PIL_beq rs1 rs2 si
+  | PIL_blt rs1 rs2 si
+  | PIL_bne rs1 rs2 si
+      => rs1 < 8 /\ rs2 < 8 /\ signed_range (32-13) si
+  | PIL_bl si
+        => signed_range (32-7) si
+  | PIL_jl i
+  | PIL_jmp i
+        => i < 2 ^ (32-7)
+  | PIL_jmpr rs1
+        => rs1 < 8
+  | PIL_ld r1 r2 i
+  | PIL_st r1 r2 i
+        => r1 < 8 /\ r2 < 8 /\ i < 2 ^ (32-13)
+  | PIL_li rd i
+        => rd < 8 /\ i < 2 ^ (32-4)
+  | PIL_InvalidI => True
+  end.
+
+(* TODO: prove these helper lemmas and add them to Picinae_theory or the coq standard lib *)
+Lemma Nshiftr_land_ones_high:
+  forall a n m, n > m -> (a << n) .& (N.ones m) = 0.
+Proof. Admitted.
+
+Lemma Nshiftr_land_high_nop:
+  forall a b n m, n > m -> (a .| b << n) .& (N.ones m) = a .& (N.ones m).
+Proof. Admitted.
+
+Lemma Nland_low:
+  forall a n, a < 2 ^ n -> a .& (N.ones n) = a.
+Proof. Admitted.
+
+Lemma xbits_lor_low:
+  forall n m i j, i <= j -> n < 2 ^ i -> xbits (n .| m) i j = xbits m i j.
+Proof. Admitted.
+
+Lemma xbits_lor_high:
+  forall n m i j, i <= j -> m = 0 \/ m >= 2 ^ j -> xbits (n .| m) i j = xbits n i j.
+Proof. Admitted.
+
+Lemma shiftr_0_or_high:
+  forall x n m, m <= n -> x << n = 0 \/ x << n >= 2 ^ m.
+Proof.
+  intros. destruct x;[left;psimpl;lia | right].
+  (* TODO: we need the N.shiftl monotonicity theorem *)
+Admitted.
+
+Lemma xbits_0_low:
+  forall n j, n < 2 ^ j -> xbits n 0 j = n.
+Proof.
+  intros; rewrite xbits_0_i; now rewrite N.mod_small.
+Qed.
+
+Theorem decode_assemble_insn :
+  forall (insn:p32_asm)
+    (WT: welltyped_p32_asm insn),
+  p32_decode (assemble_insn insn) = insn.
+Proof.
+  unfold welltyped_p32_asm, p32_decode, assemble_insn, p32_decode_op, assemble_insn_op
+    ; intros; destruct insn eqn:INSN;
+  repeat match goal with 
+  | [H: _ /\ _ |- _] => destruct H
+  end.
+  all: rewrite N.land_spec, N.ones_spec_low, Bool.andb_true_r; try lia;
+       repeat rewrite N.lor_spec; repeat rewrite N.shiftl_spec_low; try lia;
+       repeat rewrite Bool.orb_false_l; unfold N.testbit, Pos.testbit; try rewrite Bool.orb_true_l.
+  all: repeat rewrite Nshiftr_land_high_nop; try lia; simpl (_ << _ .& _); psimpl.
+  all: unfold p32_decode_binop_reg, p32_decode_binop_imm, p32_decode_cf_simm, p32_decode_imm,
+         p32_decode_reg, p32_decode_memacc, p32_decode_simm.
+  
+  (* TODO: add this xbits simplification to psimpl *)
+  all: unfold xnbits; repeat match goal with
+  | [ |- context[xbits (?N .| ?M) ?i ?j] ] => rewrite (xbits_lor_high N M i j);[
+        | solve [lia] | solve [apply shiftr_0_or_high; lia] ]
+  | [ |- context[xbits (?N .| ?M) ?i ?j] ] => rewrite (xbits_lor_low N M i j); try solve [ psimpl; lia]
+  | [ |- _ .| _ .| ?M < 2 ^ ?w ] => rewrite (lor_bound w);[|solve [lia]]
+  | [ |- _ .| ?M < 2 ^ ?w ] => apply lor_bound; try solve [psimpl ; lia]
+  (* TODO: prove the following case using the shiftr monotonicity theorem, the
+    assert by lia ensures that this case is provable and the admit is reasonable *)
+  | [ |- _ << ?S < 2 ^ ?w ] => assert (S + 3 <= w) by lia; admit 
+  end.
+  19: reflexivity.
+  5: { rewrite xbits_shiftl, xbits_shiftl; simpl (_-_) in *; psimpl;
+       rewrite xbits_0_low, xbits_0_low; try lia; reflexivity. }
+  (* TODO: psimpl does not simplify the following goal as desired:
+     PIL_li (xbits rd (1 - 1) (3 + 1 - 1)) (xbits i (4 - 4) (28 + 4 - 4)) = PIL_li rd i
+  *)
+  all: repeat rewrite xbits_shiftl; simpl (_-_) in *; psimpl.
+  all: repeat rewrite xbits_0_low; try first [ lia | reflexivity | apply ofZ_bound | now rewrite toZ_ofZ].
+Admitted.
+
+(* TODO:
+      1) define an operational semantics for PIL32_asm
+      2) define an assembly program
+      3) define small step operational semantics of the assembly program
+      4) formalize a bisimilarity between the execution of an assembly program and
+         a picinae program from a decoded assemble program given that the assembly
+         is well typed
+      5) prove it.
+*)
+
+Definition insn_length (insn:p32_asm) : N := 4.
+
+(* Each assembly code is represented as
+      
+      * a base address (e.g. 0x00100000)
+      * a list of labels (strings) and instructions (p32_asm)
+*)
+Inductive p32_assembly :=
+  P32_ASSEMBLY (base_addr:N) (code:list (sum string p32_asm)).
+  
+Fixpoint label_loc (label:string) (base_addr:N) (code:list (sum string p32_asm)) : option N :=
+  match code with
+  | nil => None
+  | inl label' :: t => if (label =? label')%string then Some base_addr 
+      else label_loc label base_addr t
+  | inr insn :: t => label_loc label (base_addr + (insn_length insn)) t
+  end.
+  
+Import ListNotations.
+Open Scope string.
+
+Definition p32_assemble_insn_bytes (insn:p32_asm) : list N :=
+  (xnbits (assemble_insn insn) 0  8) ::
+  (xnbits (assemble_insn insn) 8  8) ::
+  (xnbits (assemble_insn insn) 16 8) ::
+  (xnbits (assemble_insn insn) 24 8) :: nil.
+  
+Fixpoint p32_assemble (base_addr:N) (code:list (p32_asm)) : list (addr * N) :=
+  match code with
+  | nil => nil
+  | insn :: t => match p32_assemble_insn_bytes insn with
+    | b0 :: b1 :: b2 :: b3 :: nil =>
+      (0 + base_addr, b0) :: (1 + base_addr, b1) :: 
+      (2 + base_addr, b2) :: (3 + base_addr, b3) :: 
+      (p32_assemble (4+base_addr) t)
+    | _ => nil
+    end
+  end.
+  
+(* Definition program' := [PIL_li 0 0; PIL_addi 1 1 1; PIL_subi 2 2 1; PIL_beq 0 2 (-12)%Z]. *)
+(* Compute p32_assemble 0x00100000 program'. *)
+
+Fixpoint p32_assemble' (base_addr:N) (mem:addr->N) (code:list (p32_asm)) : addr -> N :=
+  match code with
+  | nil => mem
+  | insn :: t => p32_assemble' (base_addr+4) (setmem 32 LittleE 4 mem base_addr (assemble_insn insn)) t
+  end.
+
+(* Compute p32_assemble' 0x00100000 (fun _ => 0) program'. *)
+
+(* `assoc_list` turns a list pairing addresses and bytes into a function.
+   If the address is not set then the default byte value is 0.
+   
+   Example use:
+        
+        Definition program := [PIL_li 0 0; PIL_InvalidI].
+        assoc_list (p32_assemble 0x1000 program)
+   
+   Needing to have a default byte value is a limitation of needing to provide
+   a concrete, rather than existentially quantified, value. We can ameliorate
+   this in proofs by quantifying over memory values that exactly match the
+   behavior of the concrete memory for the addresses in which the program
+   is written.
+*)
+
+Fixpoint assoc_list (memlist:list (addr * N)) : addr -> N :=
+  match memlist with
+  | nil => fun _ => 0
+  | (addr, b) :: t => fun a => if a == addr then b else assoc_list t a
+  end.
+
+Definition p32_assemble'' (base_addr:N) (code:list p32_asm) : addr -> N :=
+  assoc_list (p32_assemble base_addr code).
+  
+
+Require Import String.
+Require Import Ascii.
+Require Import Recdef.
+Require Import Program.
+Require Import Lia.
+
+Open Scope string.
+Open Scope nat.
+Definition newline :string := String "010" EmptyString.
+
+Program Fixpoint N2str (n:nat) {measure n}: string :=
+  (match n with
+    | O => "0"
+    | _ => 
+       (if (N2str (n/10) =? "0")%string then EmptyString else N2str (n/10))
+         ++ 
+       (match n mod 10 with
+         | O => "0"
+         | 1 => "1"
+         | 2 => "2"
+         | 3 => "3"
+         | 4 => "4"
+         | 5 => "5"
+         | 6 => "6"
+         | 7 => "7"
+         | 8 => "8"
+         | 9 => "9"
+         | _ => "ERROR"
+       end)
+  end)%nat .
+Obligation 1. 
+  enough (H: fst (Nat.divmod n 9 0 9) = (n / 10));[
+  rewrite H; apply Nat.div_lt; lia| now unfold Nat.divmod]. Defined.
+Next Obligation.
+  enough (H: fst (Nat.divmod n 9 0 9) = (n / 10));[
+  rewrite H; apply Nat.div_lt; lia| now unfold Nat.divmod]. Defined.
+Next Obligation.
+  repeat (split || lia). Defined.
+Close Scope nat.
+
+Fixpoint bytematches (l:list (addr * N)) : string :=
+  match l with
+  | nil => EmptyString
+  | (a,b)::t => "  | " ++ (N2str (N.to_nat a)) ++ " => " ++ (N2str (N.to_nat b)) ++ newline
+                 ++ (bytematches t)
+  end.
+
+Definition print_code (l:list (addr * N)) (name:string) :=
+  "Definition " ++ name ++ " : addr -> N :=" ++ newline ++
+  "fun a => match a with" ++ newline ++ (bytematches l)
+  ++ "  | _ => 0" ++ newline ++ "end."
+.
